current status of ExpandWhens (still with errors because definitions are not copied automatically)

src/ExpandWhens.v
@@ -1,1587 +1,97 @@
-From Coq Require Import FunInd FMaps FMapAVL OrderedType ZArith.
-From mathcomp Require Import ssreflect ssrbool ssrnat ssrint eqtype seq ssrfun.
-From simplssrlib Require Import Types SsrOrder FSets FMaps Tactics Var Store.
+From Coq Require Import BinNat ZArith.
+From mathcomp Require Import ssreflect ssrbool eqtype seq fintype.
+From simplssrlib Require Import SsrOrder Var.
+From firrtl Require Import Env Firrtl HiEnv HiFirrtl.
+
+(* From Coq Require Import FunInd FMaps FMapAVL OrderedType ZArith.
+From mathcomp Require Import ssrnat ssrint seq ssrfun.
+From simplssrlib Require Import Types FSets FMaps Tactics Store.
 From nbits Require Import NBits.
-From firrtl Require Import Firrtl Env HiEnv.
 
 Set Implicit Arguments.
 Unset Strict Implicit.
-Import Prenex Implicits.
-
-(* Delimit Scope hifirrtl with hifirrtl. *)
-
-Section HiFirrtl.
-
-
-  (****** Syntax ******)
-
-  (****** Expressions ******)
-
-  Variable var : eqType.
-
-  Inductive sign := Unsigned | Signed.
-
-  Inductive hfexpr : Type :=
-  | Econst : fgtyp -> bits -> hfexpr
-  | Ecast : ucast -> hfexpr -> hfexpr
-  | Eprim_unop : eunop -> hfexpr -> hfexpr
-  | Eprim_binop : ebinop -> hfexpr -> hfexpr -> hfexpr
-  | Emux : hfexpr -> hfexpr -> hfexpr -> hfexpr
-  | Evalidif : hfexpr -> hfexpr -> hfexpr
-  | Eref : href -> hfexpr
-  with href : Type :=
-  | Eid : var -> href
-  | Esubfield : href -> var -> href (* HiFirrtl *)
-  | Esubindex : href -> nat -> href (* HiFirrtl *)
-  | Esubaccess : href -> hfexpr -> href (* HiFirrtl *)
-  .
-
-  (** equality of hfexpr and href are decidable *)
-  Axiom hfexpr_eq_dec : forall {x y : hfexpr}, {x = y} + {x <> y}.
-  Parameter hfexpr_eqn : forall (x y : hfexpr), bool.
-  Axiom hfexpr_eqP : Equality.axiom hfexpr_eqn.
-  Canonical hfexpr_eqMixin := EqMixin hfexpr_eqP.
-  Canonical hfexpr_eqType := Eval hnf in EqType hfexpr hfexpr_eqMixin.
-
-  Axiom href_eq_dec : forall {x y : href}, {x = y} + {x <> y}.
-  Parameter href_eqn : forall (x y : href), bool.
-  Axiom href_eqP : Equality.axiom href_eqn.
-  Canonical href_eqMixin := EqMixin href_eqP.
-  Canonical href_eqType := Eval hnf in EqType href href_eqMixin.
-
-  (****** Statements ******)
-
-  Record mem_port : Type :=
-    mk_mem_port
-      {
-        id : var;
-        addr : var;
-        en : var;
-        clk : var;
-        mask : var
-      }.
-  
-  Record hfmem : Type :=
-    mk_fmem
-      {
-        data_type : ftype;
-        depth : nat;
-        reader : seq mem_port;
-        writer : seq mem_port;
-        read_latency : nat;
-        write_latency : nat;
-        read_write : ruw
-      }.
-
-  Inductive rst : Type :=
-  | NRst : rst
-  | Rst : hfexpr -> hfexpr -> rst.
-
-  Record hfreg : Type :=
-    mk_freg
-      {
-        (* rid : var; *)
-        type : ftype;
-        clock : hfexpr;
-        reset : rst
-      }.
-
-  Definition inst_ports : Type := seq var.
-
-  Inductive hfstmt : Type :=
-  | Sskip
-  | Swire : var -> ftype -> hfstmt
-  | Sreg : var -> hfreg -> hfstmt
-  | Smem : var -> hfmem -> hfstmt
-  | Sinst : var -> var -> hfstmt
-  | Snode : var -> hfexpr -> hfstmt
-  | Sfcnct : href -> hfexpr -> hfstmt
-  | Spcnct : href -> hfexpr -> hfstmt
-  | Sinvalid : href -> hfstmt
-  (* | Sattach : seq var -> fstmt *)
-  | Swhen : hfexpr -> hfstmt_seq -> hfstmt_seq -> hfstmt
-  (* | Sstop : hfexpr -> hfexpr -> nat -> hfstmt *)
-  (* | Sprintf (* TBD *) *)
-  (* | Sassert (* TBD *) *)
-  (* | Sassume (* TBD *) *)
-  (* | Sdefname : var -> fstmt *) (* TBD *)
-  (* | Sparam : var -> fexpr -> fstmt *) (* TBD *)
-  with hfstmt_seq : Type :=
-       | Qnil
-       | Qcons : hfstmt -> hfstmt_seq -> hfstmt_seq.
-
-   Scheme hfstmt_seq_hfstmt_ind := Induction for hfstmt_seq Sort Prop
-   with hfstmt_hfstmt_seq_ind := Induction for hfstmt Sort Prop.
-
-   Definition Qhead (default : hfstmt) (s : hfstmt_seq) : hfstmt :=
-   match s with Qnil => default
-              | Qcons h tl => h end.
-
-   Fixpoint Qcat (s1 s2 : hfstmt_seq) : hfstmt_seq :=
-   match s1 with Qnil => s2
-               | Qcons h1 tl1 => Qcons h1 (Qcat tl1 s2) end.
-
-(* Fixpoint Qcatrev (s1 s2 : hfstmt_seq) : hfstmt_seq := (* calculates the reversal of s1, followed by s2 *)
-   match s1 with Qnil => s2
-               | Qcons h1 tl1 => Qcatrev tl1 (Qcons h1 s2) end.
-
-   Definition Qrev (s : hfstmt_seq) : hfstmt_seq := Qcatrev s Qnil.
-
-   Fixpoint Qfoldl {R : Type} (f : R -> hfstmt -> R) (s : hfstmt_seq) (default : R) :=
-   match s with Qnil => default
-              | Qcons h tl => Qfoldl f tl (f default h) end.
-   Fixpoint Qfoldr {R : Type} (f : hfstmt -> R -> R) (default : R) (s : hfstmt_seq) :=
-   match s with Qnil => default
-              | Qcons h tl => f h (Qfoldr f default tl) end. *)
-
-  Inductive hfport : Type :=
-  | Finput : var -> ftype -> hfport
-  | Foutput : var -> ftype -> hfport
-  .
-
-  Inductive hfmodule : Type :=
-  | FInmod : var -> seq hfport -> hfstmt_seq -> hfmodule
-  | FExmod : var -> seq hfport -> hfstmt_seq -> hfmodule
-(* DNJ: External modules do not contain statements but only an interface.
-They may contain the following special statements:
-one “defname = ...” (to set the Verilog name)
-zero, one, or multiple “parameter <variable> = <constant> (to pass parameters to the Verilog design that implements this module)
-XM : TO BE DESIGNED , how to present the parameters
-Discussion result: Because we concentrate on correctness,
-and external modules are black boxes whose behaviour is unknown,
-it does not make sense to put effort in external modules.
-*)
-  .
-
-  Inductive hfcircuit : Type := Fcircuit : var -> seq hfmodule -> hfcircuit.
-
-End HiFirrtl.
-
-
-(********************************************************************************)
-
-(** Identifiers *)
-
-(* offset of sub-elements *)
-Fixpoint size_of_ftype ft :=
-  match ft with
-  | Gtyp t => 1
-  | Atyp t n => (size_of_ftype t) * n
-  | Btyp b => size_of_fields b
-  end
-with size_of_fields b :=
-       match b with
-       | Fnil => 0
-       | Fflips v fl t fs => (size_of_ftype t) + size_of_fields fs
-       end.
-
-Fixpoint offset_of_subfield_b ft fid n :=
-  match ft with
-  | Fnil => n
-  | Fflips v fl t fs => if fid == v then n else offset_of_subfield_b fs fid (n + size_of_ftype t)
-  end.
-
-Definition offset_of_subfield ft fid n :=
-  match ft with
-  | Gtyp t => 0
-  | Atyp t n => 0
-  | Btyp b => offset_of_subfield_b b fid n
-  end.
-
-Definition offset_of_subindex ft m :=
-  match ft with
-  | Gtyp t => 0
-  | Atyp t n => m
-  | Btyp b => 0
-  end.
-
-Module Type EqNOrder <: DecidableType.
-  Parameter T : eqType.
-  Definition t : Type := T.
-  Definition eq : t -> t -> Prop := fun x y => x == y.
-  Axiom eq_refl : forall x : t, eq x x.
-  Axiom eq_sym : forall x y : t, eq x y -> eq y x.
-  Axiom eq_trans : forall x y z : t, eq x y -> eq y z -> eq x z.
-  Parameter eq_dec : forall x y : t, { eq x y } + { ~ eq x y }.
-End EqNOrder.
-  
-Module Type WFMap <: FMapInterface.WS.
-  Declare Module SE : DecidableType.
-  Module E : DecidableType
-  with Definition t := SE.t
-  with Definition eq := SE.eq
-  with Definition eq_refl := SE.eq_refl
-  with Definition eq_sym := SE.eq_sym
-  with Definition eq_trans := SE.eq_trans
-  with Definition eq_dec := SE.eq_dec
-    := SE.
-  Include WSfun E.
-End WFMap.
-
-(* make modules for paired idents*)
-Module ProdVarOrder := MakeProdOrderWithDefaultSucc VarOrder VarOrder.
-Module PVS <: SsrFSetWithNew := FSets.MakeTreeSetWithNew ProdVarOrder.
-Module PVM <: SsrFMapWithNew := FMaps.MakeTreeMapWithNew ProdVarOrder.
-Module Ids_map2 := Map2 PVS PVS.
-Module Ids_id_map2 := Map2 PVS VS.
-
-
-(********************************************************************************)
-
-(** Component Environment *)
-
-Section Component_types.
-  (* A mapping from a variable to its component type.
-  This mapping is needed because a register or memory definition
-  contains more information than just the data type. *)
-  Variable var : eqType.
-
-  Inductive cmpnt_init_typs : Type :=
-  | Aggr_typ : ftype -> cmpnt_init_typs
-  | Reg_typ : hfreg var -> cmpnt_init_typs
-  | Mem_typ : hfmem var -> cmpnt_init_typs
-  (* | Inst_typ : ftype -> seq var -> cmpnt_init_typs *)
-  | Unknown_typ : cmpnt_init_typs.
-
-  (* data type of component *)
-  Definition type_of_cmpnttyp ct :=
-    match ct with
-    | Aggr_typ t => t
-    | Reg_typ r => type r
-    | Mem_typ m => data_type m
-    | Unknown_typ => Gtyp (Fuint 0)
-    end.
-
-End Component_types.
-
-
-Module Type CmpntEnv (V : SsrOrder) <: SsrFMap.
-  (* a module interface to store components in the form a map from (defined) identifiers
-  to their data types (e.g. ``UInt<3>'') and kind (e.g. ``node''). *)
-  Include SsrFMap.
-
-  Local Notation var := V.t.
-  Local Notation cmpnttyp := (cmpnt_init_typs V.T).
-  Definition env : Type := t (cmpnttyp * fcomponent).
-  (* The default type of a variable not in the typing environment *)
-  Parameter deftyp : cmpnttyp * fcomponent.
-  (* Find the type of a variable in a typing environment.
-     If a variable is not in the typing environment, return the default type. *)
-  Parameter vtyp : SE.t -> env -> (cmpnttyp * fcomponent).
-  Axiom find_some_vtyp :
-    forall {x : SE.t} {ty :cmpnttyp * fcomponent} {e : env}, find x e = Some ty -> vtyp x e = ty.
-  Axiom find_none_vtyp :
-    forall {x : SE.t} {e : env}, find x e = None -> vtyp x e = deftyp.
-  (* Axiom vtyp_find : *)
-  (*   forall {x : SE.t} {ty : cmpnt_init_typs V.T * fcomponent} {e : env}, *)
-  (*     (vtyp x e == ty) = (find x e == Some ty) || ((find x e == None) && (ty == deftyp)). *)
-  Axiom vtyp_add_eq :
-    forall {x y : SE.t} {ty : cmpnt_init_typs V.T * fcomponent} {e : env}, x == y -> vtyp x (add y ty e) = ty.
-  Axiom vtyp_add_neq :
-    forall {x y : SE.t} {ty : cmpnt_init_typs V.T * fcomponent} {e : env},
-      x != y -> vtyp x (add y ty e) = vtyp x e.
-  Axiom not_mem_vtyp :
-    forall {v : SE.t} {e : env}, ~~ mem v e -> vtyp v e = deftyp. (* mem = member of the SsrFMap *)
-
-  (*Parameter Add : SE.t -> (cmpnttyp * fcomponent) -> env -> env -> Prop.
-  Parameter Add_add : forall v f e, Add v f e (add v f e).*)
-
-  (* Return the env with a variable v, where the fst element of type is given *)
-  Parameter add_fst : SE.t -> cmpnttyp -> env -> env.
-  Parameter Add_fst : SE.t -> cmpnttyp -> env -> env -> Prop.
-  Parameter Add_add_fst : forall v f e, Add_fst v f e (add_fst v f e).
-
-  (* Return the env with a variable v, where the snd element of type is given *)
-  Parameter add_snd : SE.t -> fcomponent -> env -> env.
-  Parameter Add_snd : SE.t -> fcomponent -> env -> env -> Prop.
-
-End CmpntEnv.
-
-Module MakeCmpntEnv (V : SsrOrder) (VM : SsrFMap with Module SE := V) <:
-  CmpntEnv V with Module SE := V.
-  (* concretisation of the above module interface
-  (in particular, defines vtyp) *)
-  Include VM.
-  Module Lemmas := FMapLemmas VM.
-  Local Notation cmpnttyp := (cmpnt_init_typs V.T).
-  (* Definition aggr_typ ty := @Aggr_typ V.T ty. *)
-  (* Definition reg_typ ty := @Reg_typ V.T ty. *)
-  (* Definition mem_typ ty := @Mem_typ V.T ty. *)
-  Definition env : Type := t (cmpnttyp * fcomponent).
-
-  (* The default type of a variable not in the typing environment *)
-  Definition deftyp := (Unknown_typ V.T, Node).
-
-  (* Find the type of a variable in a typing environment.
-     If a variable is not in the typing environment, return the default type. *)
-  Definition vtyp (v : V.t) (e : env) : cmpnttyp * fcomponent :=
-    match VM.find v e with
-    | None => deftyp
-    | Some ty => ty
-    end.
-
-  Lemma find_some_vtyp {x ty e} : find x e = Some ty -> vtyp x e = ty.
-  Proof. move=> H. rewrite /vtyp H. reflexivity. Qed.
-
-  Lemma find_none_vtyp {x e} : find x e = None -> vtyp x e = deftyp.
-  Proof. move=> H. rewrite /vtyp H. reflexivity. Qed.
-
-  Lemma vtyp_add_eq {x y ty e} : x == y -> vtyp x (add y ty e) = ty.
-  Proof. rewrite /vtyp /add => H. by rewrite (Lemmas.find_add_eq H). Qed.
-
-  Lemma vtyp_add_neq {x y ty e} : x != y -> vtyp x (add y ty e) = vtyp x e.
-  Proof.
-    move/negP=> Hxy. rewrite /vtyp /add. by rewrite (Lemmas.find_add_neq Hxy).
-  Qed.
-
-  Lemma not_mem_vtyp v e : ~~ mem v e -> vtyp v e = deftyp.
-  Proof. rewrite /vtyp => H. by rewrite Lemmas.not_mem_find_none. Qed.
-
-  (*Definition Add x c e e' := forall y, vtyp y e' = vtyp y (add x c e).
-  Lemma Add_add : forall v f e, Add v f e (add v f e).
-  Proof. done. Qed.*)
-
-  Definition add_fst (v : V.t) (c : cmpnttyp) (e : env) : env :=
-    let (f, s) := vtyp v e in add v (c, s) e.
-  Definition add_snd (v : V.t) (fc : fcomponent) (e : env) : env :=
-    let (f, s) := vtyp v e in add v (f, fc) e.
-  Definition Add_fst x c e e' := forall y, fst (vtyp y e') = fst (vtyp y (add_fst x c e)).
-  Lemma Add_add_fst {v c e} : Add_fst v c e (add_fst v c e).
-  Proof. done. Qed.
-  Definition Add_snd x c e e' := forall y, snd (vtyp y e') = snd (vtyp y (add_snd x c e)).
-  Lemma Add_add_snd {v c e} : Add_snd v c e (add_snd v c e).
-  Proof. done. Qed.
-
-End MakeCmpntEnv.
-
-
-(********************************************************************************)
-
-(** Single var, Component Environment *)
-Module CE (*<: CmpntEnv VarOrder *) := MakeCmpntEnv VarOrder VM.
-
-(** Paired var, Component Environment *)
-Module CEP  := MakeCmpntEnv ProdVarOrder PVM.
-
-(********************************************************************************)
-
-(** Component Connections *)
-
-(* rhs expressions *)
-Section Rhs_expr.
-  Variable v : eqType.
-  Inductive rhs_expr : Type :=
-  | R_fexpr : hfexpr v -> rhs_expr
-  | R_default
-  .
-
-
-  (** eq dec *)
-  Lemma rhs_expr_eq_dec : forall {x y : rhs_expr}, {x = y} + {x <> y}.
-  Proof. induction x, y ; try (right ; discriminate) ; try (left ; reflexivity).
-  case Eq: (h == h0).
-  all: move /hfexpr_eqP : Eq => Eq.
-  left ; replace h0 with h ; reflexivity.
-  right ; injection ; apply Eq.
-  Qed.
-
-  Definition rhs_expr_eqn (x y : rhs_expr) : bool :=
-  match x, y with R_fexpr e1, R_fexpr e2 => e1 == e2 | R_default, R_default => true | _, _ => false end.
-
-  Lemma rhs_expr_eqP : Equality.axiom rhs_expr_eqn.
-  Proof. unfold Equality.axiom, rhs_expr_eqn.
-  induction x, y ; try (apply ReflectF ; discriminate) ; try (apply ReflectT ; reflexivity).
-  case Eq: (h == h0).
-  all: move /hfexpr_eqP : Eq => Eq.
-  apply ReflectT ; replace h0 with h ; reflexivity.
-  apply ReflectF ; injection ; apply Eq.
-  Qed.
-
-  Canonical rhs_expr_eqMixin := EqMixin rhs_expr_eqP.
-  Canonical rhs_expr_eqType := Eval hnf in EqType rhs_expr rhs_expr_eqMixin.
-
-End Rhs_expr.
-
-(********************************************************************************)
-
-Module Type StructStore (V : SsrOrder) (CE : CmpntEnv V with Module SE := V).
-  (* extension of the component environment above
-  with functions (and lemmas) to define additional variables *)
-
-  Module Lemmas := FMapLemmas CE.
-
-  Local Notation var := V.t.
-  Local Notation value := (rhs_expr V.T).
-
-  Parameter t : Type.
-  Parameter empty : t.
-  Parameter find : var -> t -> option value.
-  Parameter map2 : (option value -> option value -> option value) -> t -> t -> t.
-  Parameter acc : var -> t -> value.
-  Parameter upd : var -> value -> t -> t.
-  Parameter upd2 : var -> value -> var -> value -> t -> t.
-  Parameter acc_upd_eq : forall {x y v s}, x == y -> acc x (upd y v s) = v.
-  Parameter find_upd_eq : forall {x y v s}, x == y -> find x (upd y v s) = Some v.
-  Parameter acc_upd_neq : forall {x y v s}, x != y -> acc x (upd y v s) = acc x s.
-  Parameter find_upd_neq : forall {x y v s}, x != y -> find x (upd y v s) = find x s.
-  Parameter acc_upd2_eq1 :
-    forall {x y1 v1 y2 v2 s},
-      x == y1 -> x != y2 -> acc x (upd2 y1 v1 y2 v2 s) = v1.
-  Parameter acc_upd2_eq2 :
-    forall {x y1 v1 y2 v2 s},
-      x == y2 -> acc x (upd2 y1 v1 y2 v2 s) = v2.
-  Parameter acc_upd2_neq :
-    forall {x y1 v1 y2 v2 s},
-      x != y1 -> x != y2 -> acc x (upd2 y1 v1 y2 v2 s) = acc x s.
-  Parameter map2_eq : forall (m m': t)
-        (x:var)(f:option value->option value->option value),
-        f None None == None ->
-        find x (map2 f m m') = f (find x m) (find x m').
-  Parameter Upd : var -> value -> t -> t -> Prop.
-  Definition Upd2 x1 v1 x2 v2 (s1 s2 : t) : Prop :=
-    forall y, acc y s2 = acc y (upd x2 v2 (upd x1 v1 s1)).
-  Parameter Equal : t -> t -> Prop.
-  Parameter Upd_upd : forall x v s, Upd x v s (upd x v s).
-  Parameter Upd2_upd :
-    forall x1 v1 x2 v2 s, Upd2 x1 v1 x2 v2 s (upd x2 v2 (upd x1 v1 s)).
-  Parameter Upd2_upd2 : forall x1 v1 x2 v2 s, Upd2 x1 v1 x2 v2 s (upd2 x1 v1 x2 v2 s).
-  Parameter acc_Upd_eq : forall x y v s1 s2, x == y -> Upd y v s1 s2 -> acc x s2 = v.
-  Parameter acc_Upd_neq :
-    forall x y v s1 s2, x != y -> Upd y v s1 s2 -> acc x s2 = acc x s1.
-  Parameter acc_Upd2_eq1 :
-    forall x y1 v1 y2 v2 s1 s2,
-      x == y1 -> x != y2 -> Upd2 y1 v1 y2 v2 s1 s2 -> acc x s2 = v1.
-  Parameter acc_Upd2_eq2 :
-    forall x y1 v1 y2 v2 s1 s2, x == y2 -> Upd2 y1 v1 y2 v2 s1 s2 -> acc x s2 = v2.
-  Parameter acc_Upd2_neq :
-    forall x y1 v1 y2 v2 s1 s2,
-      x != y1 -> x != y2 -> Upd2 y1 v1 y2 v2 s1 s2 -> acc x s2 = acc x s1.
-  Parameter Equal_def :
-    forall s1 s2,
-      Equal s1 s2 <-> (forall v, acc v s1 = acc v s2).
-  Parameter Equal_refl : forall s, Equal s s.
-  Parameter Equal_sym : forall s1 s2, Equal s1 s2 -> Equal s2 s1.
-  Parameter Equal_trans : forall s1 s2 s3, Equal s1 s2 -> Equal s2 s3 -> Equal s1 s3.
-  Parameter Equal_ST : RelationClasses.Equivalence Equal.
-  Parameter Equal_upd_Equal :
-    forall v e s1 s2, Equal s1 s2 -> Equal (upd v e s1) (upd v e s2).
-  Parameter Equal_Upd_Equal :
-    forall v e s1 s2 s3 s4,
-      Upd v e s1 s2 -> Upd v e s3 s4 -> Equal s1 s3 -> Equal s2 s4.
-  Parameter Upd_pred_Equal :
-    forall v e s1 s2 s, Upd v e s1 s2 -> Equal s1 s -> Upd v e s s2.
-  Parameter Upd_succ_Equal :
-    forall v e s1 s2 s, Upd v e s1 s2 -> Equal s2 s -> Upd v e s1 s.
-End StructStore.
-
-Module StructType (V:SsrOrder)<: HasDefaultTyp.
-  Definition t : Type := rhs_expr V.T.
-  Definition default : t := R_default V.T.
-
-End StructType.
-
-Module MakeStructStore (V : SsrOrder) (CE : CmpntEnv V with Module SE := V) <:
-  StructStore V CE.
-  Module StructTypeV := StructType V.
-  Include MakeTStoreMap V StructTypeV.
-  Module Lemmas := FMapLemmas CE.
-  Definition map2 (f : option (rhs_expr V.T) -> option (rhs_expr V.T) -> option (rhs_expr V.T)) (s1 s2 : t) : t :=
-    M.map2 f s1 s2.
-  Definition find (v: V.t) (s : t) := M.find v s.
-  Module Lemmas_M := FMapLemmas M.
-  Lemma find_upd_eq : forall {x y v s}, x == y -> find x (upd y v s) = Some v.
-  Proof.
-  intros.
-  unfold upd.
-  apply Lemmas_M.find_add_eq.
-  exact H.
-  Qed.
-  Lemma find_upd_neq : forall {x y v s}, x != y -> find x (upd y v s) = find x s.
-  Proof.
-  intros.
-  unfold upd.
-  apply Lemmas_M.find_add_neq.
-  move/eqP.
-  move/eqP: H.
-  contradiction.
-  Qed.
-  Lemma map2_eq : forall (m m': t)
-        (x:V.t)(f:option (rhs_expr V.T)->option (rhs_expr V.T)->option (rhs_expr V.T)),
-        f None None == None ->
-        find x (map2 f m m') = f (find x m) (find x m').
-  Proof.
-  intros.
-  induction (find x m) eqn: Hxm.
-  replace (Some a) with (find x m).
-  apply M.map2_1.
-  left.
-  unfold M.In, M.Raw.In0.
-  exists a.
-  apply M.find_2.
-  exact Hxm.
-  induction (find x m') eqn: Hxm'.
-  replace (None) with (find x m).
-  replace (Some a) with (find x m').
-  apply M.map2_1.
-  right.
-  unfold M.In, M.Raw.In0.
-  exists a.
-  apply M.find_2.
-  exact Hxm'.
-  induction (f None None) eqn: Hfnn.
-  contradict H.
-  move /eqP.
-  discriminate.
-  induction (find x (map2 f m m')) eqn: Hfm.
-  assert (M.In x m \/ M.In x m').
-  apply M.map2_2 with (f := f).
-  unfold M.In, M.Raw.In0.
-  exists a.
-  apply M.find_2.
-  exact Hfm.
-  destruct H0.
-  assert (~M.In x m).
-  unfold M.In, M.Raw.In0.
-  contradict Hxm.
-  destruct Hxm.
-  replace (find x m) with (Some x0).
-  discriminate.
-  symmetry.
-  apply M.find_1.
-  exact H1.
-  contradiction.
-  assert (~M.In x m').
-  unfold M.In, M.Raw.In0.
-  contradict Hxm'.
-  destruct Hxm'.
-  replace (find x m') with (Some x0).
-  discriminate.
-  symmetry.
-  apply M.find_1.
-  exact H1.
-  contradiction.
-  reflexivity.
-  Qed.
-End MakeStructStore.
-
-(********************************************************************************)
-
-(** Single var, Component Connections *)
-Module StructState := MakeStructStore VarOrder CE.
-(** Paired var, Component Connections *)
-Module StructStateP := MakeStructStore ProdVarOrder CEP.
-
-
-Module MakeHiFirrtl
-  (V : SsrOrder) (* identifier names *)
-  (VS : SsrFSet with Module SE := V)
-  (VM : SsrFMap with Module SE := V)
-  (CE : CmpntEnv V with Module SE := V)
-  (SV : StructStore V CE). (* map from names of defined identifiers to their type and kind *)
-
-  (* Local Open Scope hifirrtl. *)
-
-  Module CELemmas := FMapLemmas CE.
-  Module VSLemmas := SsrFSetLemmas VS.
-
-  Local Notation var := V.t.
-
-  Local Notation cstate := SV.t.
-  Local Notation cenv := @CE.env.
-
-  Definition econst s c := @Econst V.T s c.
-  Definition ecast u e := @Ecast V.T u e.
-  Definition eprim_unop u e := @Eprim_unop V.T u e.
-  Definition eprim_binop b e1 e2 := @Eprim_binop V.T b e1 e2.
-  Definition emux c e1 e2 := @Emux V.T c e1 e2.
-  Definition evalidif c e := @Evalidif V.T c e.
-  Definition hfexpr := hfexpr V.T.
-  Definition eref r := @Eref V.T r.
-  Definition eid v := @Eid V.T v.
-  Definition esubfield r v := @Esubfield V.T r v.
-  Definition esubindex r n := @Esubindex V.T r n.
-  Definition esubaccess r e := @Esubaccess V.T r e.
-  Definition href := href V.T.
-
-  Definition hfstmt := hfstmt V.T.
-  Definition hfstmt_seq := hfstmt_seq V.T.
-  Definition qnil := Qnil V.T.
-(*Definition qcons s ss := @Qcons V.T s ss.*)
-  Definition sskip := @Sskip V.T.
-  Definition swire v t := @Swire V.T v t.
-  Definition sreg v r := @Sreg V.T v r.
-  Definition smem v m := @Smem V.T v m.
-  Definition snode v e := @Snode V.T v e.
-  Definition sfcnct v1 v2 := @Sfcnct V.T v1 v2.
-  Definition spcnct v1 v2 := @Spcnct V.T v1 v2.
-  Definition sinvalid v1 := @Sinvalid V.T v1.
-  Definition swhen c s1 s2 := @Swhen V.T c s1 s2.
-  (* Definition sstop e1 e2 n := @Sstop V.T e1 e2 n. *)
-  Definition sinst v1 v2 := @Sinst V.T v1 v2.
-
-  Definition hfreg := @hfreg V.T.
-  Definition mk_hfreg := @mk_freg V.T.
-  Definition nrst := @NRst V.T.
-  Definition rrst e1 e2 := @Rst V.T e1 e2.
-  Definition mk_mem_port := @mk_mem_port V.T.
-  Definition mem_port := @mem_port V.T.
-  Definition hfmem := @hfmem V.T.
-  Definition mk_hfmem := @mk_fmem V.T.
-  Definition hfport := @hfport V.T.
-  Definition hinport v t := @Finput V.T v t.
-  Definition houtport v t := @Foutput V.T v t.
-  Definition hfmodule := @hfmodule V.T.
-  Definition hfinmod v ps ss := @FInmod V.T v ps ss.
-  Definition hfexmod v ps ss := @FExmod V.T v ps ss.
-  Definition hfcircuit := @hfcircuit V.T.
-
-  Definition rhs_expr := rhs_expr V.T.
-  Definition r_fexpr e := @R_fexpr V.T e.
-  Definition r_default := @R_default V.T.
-
-  (****** Oriented type ******)
-  Inductive forient : Type :=
-  | Source | Sink | Duplex | Passive | Other.
-
-  (** eq dec *)
-  Lemma forient_eq_dec : forall {x y : forient}, {x = y} + {x <> y}.
-  Proof. induction x, y ; try (right ; discriminate) ; try (left ; reflexivity). Qed.
-  Definition forient_eqn (x y : forient) : bool :=
-  match x, y with Source, Source | Sink, Sink | Duplex, Duplex | Passive, Passive | Other, Other => true
-                | _, _ => false end.
-  Lemma forient_eqP : Equality.axiom forient_eqn.
-  Proof. unfold Equality.axiom, forient_eqn. induction x, y ; try (apply ReflectF ; discriminate) ; try (apply ReflectT ; reflexivity). Qed.
-  Canonical forient_eqMixin := EqMixin forient_eqP.
-  Canonical forient_eqType := Eval hnf in EqType forient forient_eqMixin.
-
-  Definition orient_of_comp c :=
-    match c with
-    | In_port | Instanceof | Memory | Node => Source
-    (* DNJ: Not sure whether a memory should be a source. It is written like that
-    in the specificiation, but actually the data type of a memory port is a bundle
-    defined as a sink (with some fields flipped). *)
-    | Out_port => Sink
-    | Register | Wire => Duplex
-    | Fmodule => Other
-    end.
-
-  Definition valid_lhs_orient o :=
-    match o with
-    | Sink | Duplex => true
-    | _ => false
-    end.
-
-  Definition valid_rhs_orient o :=
-    match o with
-    | Source | Duplex | Passive => true
-    | _ => false
-    end.
-
-  (* rhs expr has right orient *)
-  Fixpoint valid_rhs_ref (e : href) (ce : cenv) :=
-    match e with
-    | Eid r => let (_,c) := CE.vtyp r ce in valid_rhs_orient (orient_of_comp c)
-    | Esubfield r _ => valid_rhs_ref r ce
-    (* DNJ: Subfields can be flipped. So one needs to check with the data type of r *)
-    | Esubindex r _ => valid_rhs_ref r ce
-    | Esubaccess r _ => valid_rhs_ref r ce
-    end.
-
-  Fixpoint valid_rhs_fexpr (e : hfexpr) (ce : cenv) :=
-    match e with
-    | Econst _ _ => true
-    | Eref r => valid_rhs_ref r ce
-    | Ecast _ _ => true
-    | Eprim_binop _ _ _ => true
-    | Eprim_unop _ _ => true
-    (* DNJ: The arguments of a multiplexer or a validif need to be passive. *)
-    | Emux _ e1 e2 => valid_rhs_fexpr e1 ce && (valid_rhs_fexpr e2 ce)
-    | Evalidif _ e => valid_rhs_fexpr e ce
-    end.
-
-  Definition valid_rhs (re : rhs_expr) (ce : cenv) : bool :=
-    match re with
-    | R_default => true
-    (* | R_ftype t => is_passive t *)
-    | R_fexpr e => valid_rhs_fexpr e ce
-    (* | R_fstmt s => match s with *)
-    (*                | Sreg _ _ | Smem _ _ => true *)
-    (*                | _ => false *)
-    (*                end *)
-    end.
-
-  (****** Semantics ******)
-
-  (* ground type equivalence *)
-  Definition fgtyp_equiv t1 t2 :=
-    match t1, t2 with
-    | Fuint _, Fuint _
-    | Fsint _, Fsint _
-    | Fclock, Fclock
-    | Freset, Freset
-    (* | Freset, Fuint 1 *)
-    | Fasyncreset, Fasyncreset => true
-    | _, _ => false
-    end.
-
-  (* type equivalence *)
-  Fixpoint ftype_equiv t1 t2 :=
-    match t1, t2 with
-    | Gtyp gt1, Gtyp gt2 => fgtyp_equiv gt1 gt2
-    | Atyp t1 n1, Atyp t2 n2 => (n1 == n2) && ftype_equiv t1 t2
-    | Btyp bt1, Btyp bt2 => fbtyp_equiv bt1 bt2
-    | _, _ => false
-    end
-  with fbtyp_equiv bt1 bt2 :=
-         match bt1, bt2 with
-         | Fnil, Fnil => true
-         | Fflips v1 Flipped t1 fs1, Fflips v2 Flipped t2 fs2 =>
-           (v1 == v2) && ftype_equiv t1 t2 && fbtyp_equiv fs1 fs2
-         | Fflips v1 Nflip t1 fs1, Fflips v2 Nflip t2 fs2 =>
-           (v1 == v2) && ftype_equiv t1 t2 && fbtyp_equiv fs1 fs2
-         | _, _ => false
-         end.
-
-  (* type weak equivalence *)
-  Fixpoint have_field bs f : bool :=
-    match bs with
-    | Fflips v fp t bs' => if v == f then true else have_field bs' f
-    | Fnil => false
-    end.
-
-  Fixpoint orient_of_field bs f : option fflip :=
-    match bs with
-    | Fflips v fp t bs' => if v == f then Some fp else orient_of_field bs' f
-    | Fnil => None
-    end.
-
-  Fixpoint type_of_field bs f : option ftype :=
-    match bs with
-    | Fflips v fp t bs' => if v == f then Some t else type_of_field bs' f
-    | Fnil => None
-    end.
-
-  Definition same_ffilp f1 f2 : bool :=
-    match f1, f2 with
-    | Flipped, Flipped => true
-    | Nflip, Nflip => true
-    | _, _ => false
-    end.
-
-  Fixpoint fbtyp_weak_equiv b1 b2 :=
-    match b1 with
-    | Fflips v1 fp1 t1 fs1 =>
-      match orient_of_field b1 v1, type_of_field b2 v1 with
-      | Some fp2, Some t2 => (same_ffilp fp1 fp2 && (ftype_equiv t1 t2))
-      | _, _ => fbtyp_weak_equiv fs1 b2
-      end
-    | Fnil => true
-    end.
-
-  Definition ftype_weak_equiv t1 t2 :=
-    match t1, t2 with
-    | Gtyp gt1, Gtyp gt2 => fgtyp_equiv gt1 gt2
-    | Atyp t1 n1, Atyp t2 n2 => ftype_equiv t1 t2
-    | Btyp bt1, Btyp bt2 => fbtyp_weak_equiv bt1 bt2
-    | _, _ => false
-    end.
-
-  Definition cmpnt_init_typs := @cmpnt_init_typs V.T.
-  Definition aggr_typ t := @Aggr_typ V.T t.
-  Definition reg_typ t := @Reg_typ V.T t.
-  Definition mem_typ t := @Mem_typ V.T t.
-  Definition unknown_typ := @Unknown_typ V.T.
-
-
-
-  Fixpoint eref_has_v (v:var) r :=
-    match r with
-    | Eid v1 => v1 == v
-    | Esubfield r f => eref_has_v v r
-    | Esubindex r n => eref_has_v v r
-    | Esubaccess r a => eref_has_v v r
-    end.
-
-  Fixpoint fexpr_has_v v e :=
-    match e with
-    | Econst _ _ => false
-    | Ecast _ e => fexpr_has_v v e
-    | Eprim_binop b e1 e2 => fexpr_has_v v e1 || fexpr_has_v v e2
-    | Eprim_unop u e => fexpr_has_v v e
-    | Emux c e1 e2 => fexpr_has_v v c || fexpr_has_v v e1 || fexpr_has_v v e2
-    | Evalidif c e => fexpr_has_v v c || fexpr_has_v v e
-    | Eref r => eref_has_v v r
-    end.
-
-  (********************************************************************************)
-
-  (** Pass Resolvekinds *)
-
-  (* Resolve component kind from statement, init with unknown type *)
-  Inductive resolveKinds_stmt : hfstmt -> cenv -> cenv -> Prop :=
-  | Resolve_wire v t (ce : cenv) (ce' : cenv) :
-      CE.find v ce' = Some (unknown_typ, Wire) ->
-      resolveKinds_stmt (swire v t) ce ce'
-  | Resolve_reg v r ce ce' :
-      CE.find v ce' = Some (unknown_typ, Register) ->
-      resolveKinds_stmt (sreg v r) ce ce'
-  | Resolve_inst v1 v2 ce ce' :
-  (*~~ (v1 == v2) ->*)
-      CE.find v1 ce' = Some (unknown_typ, Instanceof) ->
-      resolveKinds_stmt (sinst v1 v2) ce ce'
-  | Resolve_node v e ce ce' :
-      CE.find v ce' = Some (unknown_typ, Node) ->
-      resolveKinds_stmt (snode v e) ce ce'
-  | Resolve_mem v m ce ce' :
-      CE.find v ce' = Some (unknown_typ, Memory) ->
-      resolveKinds_stmt (smem v m) ce ce'
-  | Resolve_invalid v ce :
-      resolveKinds_stmt (sinvalid v) ce ce
-  | Resolve_skip ce :
-      resolveKinds_stmt sskip ce ce
-  | Resolve_fcnct r e ce :
-      resolveKinds_stmt (sfcnct r e) ce ce
-  | Resolve_pcnct r e ce :
-      resolveKinds_stmt (spcnct r e) ce ce
-  | Resolve_when e s1 s2 ce ce' ce'' :
-      resolveKinds_stmts s1 ce ce' ->
-      resolveKinds_stmts s2 ce' ce'' ->
-      resolveKinds_stmt (swhen e s1 s2) ce ce''
-  (* | Resolve_stop e1 e2 n ce : *)
-  (*     resolveKinds_stmt (sstop e1 e2 n) ce ce *)
-
-
-  with resolveKinds_stmts : hfstmt_seq -> cenv -> cenv -> Prop :=
-  | Resolve_stmts_nil ce :
-      resolveKinds_stmts qnil ce ce
-  | Resolve_stmts_cons s ss ce ce' ce'' :
-      resolveKinds_stmt s ce ce' ->
-      resolveKinds_stmts ss ce' ce'' ->
-    resolveKinds_stmts (Qcons s ss) ce ce''
-  .
-
-  Inductive resolveKinds_port : hfport -> CE.env -> CE.env -> Prop :=
-  | Resolve_input v t ce ce' :
-      CE.find v ce' = Some (unknown_typ, In_port) ->
-      resolveKinds_port (Finput v t) ce ce'
-  | Resolve_output v t ce ce' :
-      CE.find v ce' = Some (unknown_typ, Out_port) ->
-      resolveKinds_port (Foutput v t) ce ce'
-  .
-
-  Inductive resolveKinds_ports : seq hfport -> CE.env -> CE.env -> Prop :=
-  | Resolve_ports_nil ce :
-      resolveKinds_ports [::] ce ce
-  | Resolve_ports_cons p ps ce ce' ce'' :
-      resolveKinds_port p ce ce' ->
-      resolveKinds_ports ps ce' ce'' ->
-      resolveKinds_ports (p::ps) ce ce''.
-
-  Inductive resolveKinds_module : hfmodule -> CE.env -> CE.env -> Prop :=
-  | Resolves_inmod vm ps ss ce ce' :
-      CE.find vm ce' = Some (unknown_typ, Fmodule) ->
-      resolveKinds_module (hfinmod vm ps ss) ce ce'
-  | Resolves_exmod vm ps ss ce ce' :
-      CE.find vm ce' = Some (unknown_typ, Fmodule) ->
-      resolveKinds_module (hfexmod vm ps ss) ce ce'
-  .
-
-  Inductive resolveKinds_modules : seq hfmodule -> CE.env -> CE.env -> Prop :=
-  | Resolve_modules_nil ce :
-      resolveKinds_modules [::] ce ce
-  | Resolve_modules_cons p ps ce ce' ce'' :
-      resolveKinds_module p ce ce' ->
-      resolveKinds_modules ps ce' ce'' ->
-      resolveKinds_modules (p :: ps) ce ce''.
-
-  (* For error checking, one could replace CE.add by a function that generates an error message
-     if an identifier was already declared earlier.  However, one has to be careful about namespaces. *)
-
-  Fixpoint resolveKinds_stmt_fun (st : hfstmt) (ce : cenv) : cenv :=
-    match st with
-    | Sskip => ce
-    | Swire v t => CE.add v (unknown_typ, Wire) ce
-    | Sreg v r => CE.add v (unknown_typ, Register) ce
-    | Smem v m => CE.add v (unknown_typ, Memory) ce
-    | Sinst v m => CE.add v (unknown_typ, Instanceof) ce
-    | Snode v e => CE.add v (unknown_typ, Node) ce
-    | Sfcnct _ _
-    | Spcnct _ _
-    | Sinvalid _ => ce
-    | Swhen _ sts_true sts_false => resolveKinds_stmts_fun sts_false (resolveKinds_stmts_fun sts_true ce)
-    end
-
-  with resolveKinds_stmts_fun (sts : hfstmt_seq) (ce : cenv) : CE.env := (*fold_right resolveKinds_stmt_fun ce sts.*)
-    match sts with
-    | Qnil => ce
-    | Qcons s stl => resolveKinds_stmts_fun stl (resolveKinds_stmt_fun s ce)
-    end.
-
-  Definition resolveKinds_port_fun p ce :=
-    match p with
-    | Finput v t => CE.add v (unknown_typ, In_port) ce
-    | Foutput v t => CE.add v (unknown_typ, Out_port) ce
-    end.
-
-  Fixpoint resolveKinds_ports_fun ps ce := (*fold_right resolveKinds_port_fun ce ps.*)
-    match ps with
-    | nil => ce
-    | s :: stl => resolveKinds_ports_fun stl (resolveKinds_port_fun s ce)
-    end.
-
-  Definition resolveKinds_module_fun m ce :=
-    match m with
-    | FInmod v ps ss => CE.add v (unknown_typ, Fmodule) ce
-    | FExmod v ps ss => CE.add v (unknown_typ, Fmodule) ce
-    end.
-
-  Fixpoint resolveKinds_modules_fun ms ce := (*fold_right resolveKinds_module_fun ce ms.*)
-    match ms with
-    | nil => ce
-    | s :: stl => resolveKinds_modules_fun stl (resolveKinds_module_fun s ce)
-    end.
-
-  (******lemma of resolvekinds *****)
-  Lemma resolveKinds_snode_sem_conform :
-  forall v e ce0 ,
-    resolveKinds_stmt (Snode v e) ce0 (resolveKinds_stmt_fun (Snode v e) ce0).
-Proof.
-  intros. apply Resolve_node.
-  rewrite /resolveKinds_stmt_fun /CE.add_fst (CELemmas.add_eq_o _ _ (eq_refl v)) //.
-  Qed.
-
-Lemma resolveKinds_sreg_sem_conform :
-  forall v e ce0 ,
-  resolveKinds_stmt (Sreg v e) ce0 (resolveKinds_stmt_fun (Sreg v e) ce0).
-Proof.
-  intros. apply Resolve_reg.
-  rewrite /resolveKinds_stmt_fun /CE.add_fst (CELemmas.add_eq_o _ _ (eq_refl v)) //.
-  Qed.
-
-Lemma resolveKinds_smem_sem_conform :
-  forall v e ce0 ,
-  resolveKinds_stmt (Smem v e) ce0 (resolveKinds_stmt_fun (Smem v e) ce0).
-Proof.
-  intros. apply Resolve_mem.
-  rewrite /resolveKinds_stmt_fun /CE.add_fst (CELemmas.add_eq_o _ _ (eq_refl v)) //.
-Qed.
-
-Lemma resolveKinds_sinvalid_sem_conform :
-  forall v ce0 ,
-  resolveKinds_stmt (Sinvalid v) ce0 (resolveKinds_stmt_fun (Sinvalid v) ce0).
-Proof.
-  intros. apply Resolve_invalid.
-Qed.
-
-Lemma resolveKinds_sskip_sem_conform :
-  forall ce0 ,
-  resolveKinds_stmt sskip ce0 (resolveKinds_stmt_fun sskip ce0).
-Proof.
-  intros. apply Resolve_skip.
-Qed.
-
-Lemma resolveKinds_sfcnct_sem_conform :
-  forall r e ce0 ,
-  resolveKinds_stmt (sfcnct r e) ce0 (resolveKinds_stmt_fun (sfcnct r e) ce0).
-Proof.
-  intros. apply Resolve_fcnct.
-Qed.
-
-Lemma resolveKinds_spcnct_sem_conform :
-forall r e ce0 ,
-  resolveKinds_stmt (spcnct r e) ce0 (resolveKinds_stmt_fun (spcnct r e) ce0).
-Proof.
-  intros. apply Resolve_pcnct.
-Qed.
-
-Lemma resolveKinds_swhen_sem_conform :
-forall (e : hfexpr) (s1 s2 : hfstmt_seq) (ce0 ce1 ce2: cenv),
-  resolveKinds_stmts s1 ce0 ce1 ->
-  resolveKinds_stmts s2 ce1 (resolveKinds_stmt_fun (swhen e s1 s2) ce0) ->
-  resolveKinds_stmt (swhen e s1 s2) ce0 (resolveKinds_stmt_fun (swhen e s1 s2) ce0).
-Proof.
-  intros. apply Resolve_when with (ce' := ce1). exact H. exact H0.
-Qed.
-
-(* Lemma resolveKinds_sstop_sem_conform : *)
-(* forall e1 e2 n ce0 , *)
-(*   resolveKinds_stmt (sstop e1 e2 n) ce0 (resolveKinds_stmt_fun (sstop e1 e2 n) ce0). *)
-(* Proof. *)
-(*   intros. apply Resolve_stop. *)
-(* Qed. *)
-
-Lemma resolveKinds_swire_sem_conform :
-  forall v e ce0 ,
-  resolveKinds_stmt (Swire v e) ce0 (resolveKinds_stmt_fun (Swire v e) ce0).
-Proof.
-  intros. apply Resolve_wire.
-  rewrite /resolveKinds_stmt_fun.
-  rewrite (CELemmas.add_eq_o _ _ (eq_refl v)) //.
-Qed.
-
-Lemma resolveKinds_sinst_sem_conform :
-  forall v1 v2 ce0 ,
-  resolveKinds_stmt (Sinst v1 v2) ce0 (resolveKinds_stmt_fun (Sinst v1 v2) ce0).
-Proof.
-  intros. apply Resolve_inst.
-  rewrite /resolveKinds_stmt_fun /CE.add_fst (CELemmas.add_eq_o _ _ (eq_refl v1)) //.
-Qed.
-
-Definition resolveKinds_stmts_sem_conform_statement (sts : hfstmt_seq) : Prop :=
-forall ce0 : cenv,
-  resolveKinds_stmts sts ce0 (resolveKinds_stmts_fun sts ce0).
-
-Lemma resolveKinds_stmts_sem_conform :
-  forall sts : hfstmt_seq, resolveKinds_stmts_sem_conform_statement sts.
-Proof.
-  apply hfstmt_seq_hfstmt_ind with (P := resolveKinds_stmts_sem_conform_statement)
-                                   (P0 := fun st : hfstmt => match st with Swhen c s1 s2 => resolveKinds_stmts_sem_conform_statement s1 /\ resolveKinds_stmts_sem_conform_statement s2 | _ => True end) ; try done.
-  unfold resolveKinds_stmts_sem_conform_statement. apply Resolve_stmts_nil.
-  intros.
-  unfold resolveKinds_stmts_sem_conform_statement.
-  intros.
-  apply Resolve_stmts_cons with (ce' := resolveKinds_stmt_fun h ce0).
-  induction h.
-  - apply resolveKinds_sskip_sem_conform.
-  - apply resolveKinds_swire_sem_conform.
-  - apply resolveKinds_sreg_sem_conform.
-  - apply resolveKinds_smem_sem_conform.
-  - apply resolveKinds_sinst_sem_conform.
-  - apply resolveKinds_snode_sem_conform.
-  - apply resolveKinds_sfcnct_sem_conform.
-  - apply resolveKinds_spcnct_sem_conform.
-  - apply resolveKinds_sinvalid_sem_conform.
-  - apply resolveKinds_swhen_sem_conform with (ce1 := resolveKinds_stmts_fun h1 ce0) ; try done.
-    apply H. apply H.
-  rewrite /=.
-  apply (H0 (resolveKinds_stmt_fun h ce0)).
-  Qed.
-
-Lemma resolveKinds_inport_sem_conform :
-  forall v t ce0 ,
-    resolveKinds_port (Finput v t) ce0 (resolveKinds_port_fun (Finput v t) ce0).
-  Proof.
-    intros.
-    apply Resolve_input; try done.
-    rewrite /resolveKinds_port_fun /CE.add_fst (CELemmas.add_eq_o _ _ (eq_refl v)) //.
-    Qed.
-
-Lemma resolveKinds_outport_sem_conform :
-  forall v t ce0 ,
-    resolveKinds_port (Foutput v t) ce0 (resolveKinds_port_fun (Foutput v t) ce0).
-  Proof.
-    intros.
-    apply Resolve_output; try done.
-    rewrite /resolveKinds_port_fun /CE.add_fst (CELemmas.add_eq_o _ _ (eq_refl v)) //.
-    Qed.
-
-Lemma resolveKinds_ports_sem_conform :
-  forall ps ce0 ,
-    resolveKinds_ports ps ce0 (resolveKinds_ports_fun ps ce0).
-  Proof.
-    elim. intros. apply Resolve_ports_nil.
-    intros.
-    apply Resolve_ports_cons with (resolveKinds_port_fun a ce0).
-    elim a; intros;try done.
-    - apply resolveKinds_inport_sem_conform.
-    - apply resolveKinds_outport_sem_conform.
-    rewrite /=.
-    apply (H (resolveKinds_port_fun a ce0)).
-  Qed.
-
-Lemma resolveKinds_inmod_sem_conform :
-forall vm ps ss ce,
-  resolveKinds_module (FInmod vm ps ss) ce (resolveKinds_module_fun (FInmod vm ps ss) ce).
-Proof.
-  intros.
-  apply Resolves_inmod.
-  rewrite /resolveKinds_module_fun.
-  rewrite /CE.add_fst (CELemmas.add_eq_o _ _ (eq_refl vm)) //.
-Qed.
-
-Lemma resolveKinds_exmod_sem_conform :
-forall vm ps ss ce,
-  resolveKinds_module (FExmod vm ps ss) ce (resolveKinds_module_fun (FExmod vm ps ss) ce).
-Proof.
-  intros.
-  apply Resolves_exmod.
-  rewrite /resolveKinds_module_fun.
-  rewrite /CE.add_fst (CELemmas.add_eq_o _ _ (eq_refl vm)) //.
-Qed.
-
-Lemma resolveKinds_mods_sem_conform :
-forall ms ce0 ,
-  resolveKinds_modules ms ce0 (resolveKinds_modules_fun ms ce0).
-Proof.
-    elim. intros. apply Resolve_modules_nil.
-    intros.
-    apply Resolve_modules_cons with (resolveKinds_module_fun a ce0).
-    elim a; intros;try done.
-    - apply resolveKinds_inmod_sem_conform.
-    - apply resolveKinds_exmod_sem_conform.
-    rewrite /=.
-    apply (H (resolveKinds_module_fun a ce0)).
-    Qed.
-
-  (** decide the type and width of hifirrtl expressions *)
-
-  Parameter v2var : V.t -> Var.var.
-
-  Definition def_ftype := Gtyp (Fuint 0).
-
-  (* type of mux expression *)
-  Fixpoint mux_types t1 t2 : ftype :=
-      match t1, t2 with
-      | Gtyp (Fuint w1), Gtyp (Fuint w2) => (Gtyp (Fuint (maxn w1 w2)))
-      | Gtyp (Fsint w1), Gtyp (Fsint w2) => (Gtyp (Fsint (maxn w1 w2)))
-      | Gtyp Fclock, Gtyp Fclock => (Gtyp Fclock)
-      | Atyp t1 n1, Atyp t2 n2 => if n1 == n2 then (Atyp (mux_types t1 t2) n1)
-                                  else def_ftype
-      | Btyp bs1, Btyp bs2 => match mux_btyps bs1 bs2 with
-                              | Fnil => def_ftype
-                              | t => Btyp t
-                              end
-      | _, _ => def_ftype
-      end
-  with mux_btyps bs1 bs2 : ffield :=
-         match bs1, bs2 with
-         | Fnil, Fnil => (Fnil)
-         | Fflips v1 Nflip t1 fs1, Fflips v2 Nflip t2 fs2 =>
-           if v1 == v2 then
-             (Fflips v1 Nflip (mux_types t1 t2) (mux_btyps fs1 fs2))
-           else Fnil
-         | _, _ => Fnil
-    end.
-
-  (* type of ref expressions *)
-  Fixpoint type_of_ref r ce : ftype :=
-    match r with
-    | Eid v => type_of_cmpnttyp (fst (CE.vtyp v ce))
-    | Esubfield r v => let t := type_of_ref r ce in
-                       match t with
-                       | Btyp fs => let fix aux fx := (
-                                          match fx with
-                                          | Fflips v' f t fxs =>
-                                            if (v2var v == v') then t
-                                            else aux fxs
-                                          | Fnil => def_ftype
-                                          end )
-                                    in aux fs
-                       | _ => def_ftype
+Import Prenex Implicits. *)
+
+Include HiF.
+
+(* DNJ: What follows is my proposal to create a unique lowered index from a (high-level) reference.
+   I do not know whether this is compatible with ExpandConnects or LowerTypes. *)
+
+Open Scope N_scope.
+
+(* A bijection between pairs of natural numbers and natural numbers *)
+Definition pair (x y : N) : N :=
+   (x + y) * (x + y + 1) / 2 + x.
+
+Definition proj1 (p : N) : N :=
+   let x_plus_y := (N.sqrt (8 * p + 1) - 1) / 2 (* rounded down *) in
+   p - (x_plus_y * (x_plus_y + 1) / 2).
+
+Definition proj2 (p : N) : N :=
+   let x_plus_y := (N.sqrt (8 * p + 1) - 1) / 2 (* rounded down *) in
+   (* x_plus_y - (proj1 p), which simplifies to: *)
+   x_plus_y * (x_plus_y + 3) / 2 - p.
+
+(* pair and (proj1, proj2) are each other's inverse functions. *)
+Lemma sqrt_spec : forall n: N, N.sqrt (n * n) = n.
+Admitted. (* probably the proof can be based on something like
+   forall p: positive, Pos.sqrtrem (p * p) = (p, IsNul). *)
+
+Lemma proj1_pair : forall (x y : N), x = proj1 (pair x y).
+Admitted.
+
+Lemma proj2_pair : forall (y x : N), y = proj2 (pair x y).
+Admitted.
+
+Lemma pair_proj : forall p : N, p = pair (proj1 p) (proj2 p).
+Admitted.
+
+(* mapping from a href that is not a subaccess to an index in CE.env *)
+Fixpoint ref2var (ref : href) : N :=
+match ref with
+| Eid v => v * 3 + 1
+| Esubfield ref0 v => match ref2var ref0 with
+                      | 0 => 0
+                      | n => (pair n v) * 3 + 2
+                      end
+| Esubindex ref0 i => match ref2var ref0 with
+                      | 0 => 0
+                      | n => (pair n (N.of_nat i)) * 3 + 3
+                      end
+| Esubaccess _ _ => 0 (* cannot be translated actually *)
+end.
+
+(* mapping from an index in CE.env to a href. *)
+
+Definition to_var (n : N) : VarOrder.T := n.
+
+Fixpoint var2ref' (depth : nat) (n : N) : option href :=
+   match depth, n with
+   | 0%nat, _ | _, 0 => None
+   | S d', _ => match n mod 3 with
+                | 1 => Some (Eid (to_var ((n - 1) / 3)))
+                | 2 => let p := (n - 2) / 3 in
+                       match var2ref' d' (proj1 p) with
+                       | None => None
+                       | Some ref => Some (Esubfield ref (proj2 p))
                        end
-    | Esubindex r n => let t := type_of_ref r ce in
-                       match t with
-                       | Atyp ty n => ty
-                       | _ => def_ftype
+                | _ => let p := (n - 3) / 3 in
+                       match var2ref' d' (proj1 p) with
+                       | None => None
+                       | Some ref => Some (Esubindex ref (N.to_nat (proj2 p)))
                        end
-    | Esubaccess r e => let t := type_of_ref r ce in
-                        match t with
-                        | Atyp ty n => ty
-                        | _ => def_ftype
-                        end
-    end.
+                end
+   end.
 
-  Fixpoint base_ref r : V.t :=
-    match r with
-    | Eid v => v
-    | Esubfield r v => base_ref r
-    | Esubindex r n => base_ref r
-    | Esubaccess r n => base_ref r
-    end.
+Definition var2ref (n : N) : option href := var2ref' (N.to_nat n) n.
 
-  Fixpoint base_type_of_ref r ce : ftype :=
-    match r with
-    | Eid v => type_of_cmpnttyp (fst (CE.vtyp v ce))
-    | Esubfield r v => base_type_of_ref r ce
-    | Esubindex r n => base_type_of_ref r ce
-    | Esubaccess r n => base_type_of_ref r ce
-    end.
+Close Scope N_scope.
 
-  (* type of expression *)
-  Fixpoint type_of_hfexpr (e : hfexpr) (ce : cenv) : ftype :=
-    match e with
-    | Econst t bs => Gtyp t
-    | Eref r => type_of_ref r ce
-    | Ecast AsUInt e1 => let t := type_of_hfexpr e1 ce in
-                         match t with
-                         | Gtyp (Fsint w) | Gtyp (Fuint w) => Gtyp (Fuint w)
-                         | Gtyp Fclock => Gtyp (Fuint 1)
-                         | Gtyp Freset => Gtyp (Fuint 1)
-                         | Gtyp Fasyncreset => Gtyp (Fuint 1)
-                         | _ => def_ftype
-                         end
-    | Ecast AsSInt e1 => let t := type_of_hfexpr e1 ce in
-                         match t with
-                         | Gtyp (Fsint w) | Gtyp (Fuint w) => Gtyp (Fsint w)
-                         | Gtyp Fclock => Gtyp (Fsint 1)
-                         | Gtyp Freset => Gtyp (Fuint 1)
-                         | Gtyp Fasyncreset => Gtyp (Fuint 1)
-                         | _ => def_ftype
-                         end
-    | Ecast AsClock e1 => let t := type_of_hfexpr e1 ce in
-                          match t with
-                          | Gtyp _ =>  Gtyp Fclock
-                          | _ => def_ftype
-                          end
-    | Ecast AsReset e1 => let t := type_of_hfexpr e1 ce in
-                          match t with
-                          | Gtyp _ =>  Gtyp Freset
-                          | _ => def_ftype
-                          end
-    | Ecast AsAsync e1 => let t := type_of_hfexpr e1 ce in
-                          match t with
-                          | Gtyp _ =>  Gtyp Fasyncreset
-                          | _ => def_ftype
-                          end
-    | Eprim_unop (Upad n) e1 => let t := type_of_hfexpr e1 ce in
-                                match t with
-                                | Gtyp (Fsint w) => Gtyp (Fsint (maxn w n))
-                                | Gtyp (Fuint w) => Gtyp (Fuint (maxn w n))
-                                | _ => def_ftype
-                                end
-    | Eprim_unop (Ushl n) e1 => let t := type_of_hfexpr e1 ce in
-                                match t with
-                                | Gtyp (Fsint w) => Gtyp (Fsint (w + n))
-                                | Gtyp (Fuint w) => Gtyp (Fuint (w + n))
-                                | _ => def_ftype
-                                end
-    | Eprim_unop (Ushr n) e1 => let t := type_of_hfexpr e1 ce in
-                                match t with
-                                | Gtyp (Fsint w) => if n < w then Gtyp (Fsint (maxn (w - n) 1))
-                                                    else Gtyp (Fuint 1)
-                                | Gtyp (Fuint w) => if n < w then Gtyp (Fuint (maxn (w - n) 1))
-                                                    else Gtyp (Fuint 1)
-                                | _ => def_ftype
-                                end
-    | Eprim_unop Ucvt e1 => let t := type_of_hfexpr e1 ce in
-                                match t with
-                                | Gtyp (Fsint w) => Gtyp (Fsint w)
-                                | Gtyp (Fuint w) => Gtyp (Fsint (w + 1))
-                                | _ => def_ftype
-                                end
-    | Eprim_unop Uneg e1 => let t := type_of_hfexpr e1 ce in
-                                match t with
-                                | Gtyp (Fsint w) | Gtyp (Fuint w) => Gtyp (Fsint (w + 1))
-                                | _ => def_ftype
-                                end
-    | Eprim_unop Unot e1 => let t := type_of_hfexpr e1 ce in
-                                match t with
-                                | Gtyp (Fsint w) | Gtyp (Fuint w) => Gtyp (Fuint w)
-                                | _ => def_ftype
-                                end
-    | Eprim_unop (Uextr n1 n2) e1 => let t := type_of_hfexpr e1 ce in
-                                     match t with
-                                     | Gtyp (Fsint w) | Gtyp (Fuint w) =>
-                                                        if (n2 <= n1) && (n1 < w) then Gtyp (Fuint (n1 - n2 + 1))
-                                                        else def_ftype
-                                     | _ => def_ftype
-                                     end
-    | Eprim_unop (Uhead n) e1 => let t := type_of_hfexpr e1 ce in
-                                 match t with
-                                 | Gtyp (Fsint w) | Gtyp (Fuint w) =>
-                                                    if n <= w then Gtyp (Fuint n)
-                                                    else def_ftype
-                                 | _ => def_ftype
-                                 end
-    | Eprim_unop (Utail n) e1 => let t := type_of_hfexpr e1 ce in
-                                 match t with
-                                 | Gtyp (Fsint w) | Gtyp (Fuint w) =>
-                                                    if n <= w then Gtyp (Fuint (w - n))
-                                                    else def_ftype
-                                 | _ => def_ftype
-                                 end
-    | Eprim_unop _ e1 => let t := type_of_hfexpr e1 ce in
-                         match t with
-                         | Gtyp (Fsint _) | Gtyp (Fuint _) => Gtyp (Fuint 1)
-                         | _ => def_ftype
-                         end
-    | Eprim_binop (Bcomp _) e1 e2 => let t1 := type_of_hfexpr e1 ce in
-                                     let t2 := type_of_hfexpr e2 ce in
-                                     match t1, t2 with
-                                     | Gtyp (Fsint _), Gtyp (Fsint _)
-                                     | Gtyp (Fuint _), Gtyp (Fuint _) => Gtyp (Fuint 1)
-                                     | _, _ => def_ftype
-                                     end
-    | Eprim_binop Badd e1 e2
-    | Eprim_binop Bsub e1 e2 => let t1 := type_of_hfexpr e1 ce in
-                                let t2 := type_of_hfexpr e2 ce in
-                                match t1, t2 with
-                                | Gtyp (Fuint w1) , Gtyp (Fuint w2) => Gtyp (Fuint (maxn w1 w2 + 1))
-                                | Gtyp (Fsint w1) , Gtyp (Fsint w2) => Gtyp (Fsint (maxn w1 w2 + 1))
-                                | _, _ => def_ftype
-                                end
-    | Eprim_binop Bmul e1 e2 => let t1 := type_of_hfexpr e1 ce in
-                                let t2 := type_of_hfexpr e2 ce in
-                                match t1, t2 with
-                                | Gtyp (Fuint w1) , Gtyp (Fuint w2) => Gtyp (Fuint (w1 + w2))
-                                | Gtyp (Fsint w1) , Gtyp (Fsint w2) => Gtyp (Fsint (w1 + w2))
-                                | _, _ => def_ftype
-                                end
-    | Eprim_binop Bdiv e1 e2  => let t1 := type_of_hfexpr e1 ce in
-                                 let t2 := type_of_hfexpr e2 ce in
-                                 match t1, t2 with
-                                 | Gtyp (Fuint w1), Gtyp (Fuint w2) => Gtyp (Fuint w1)
-                                 | Gtyp (Fsint w1), Gtyp (Fsint w2) => Gtyp (Fsint (w1 + 1))
-                                 | _, _ => def_ftype
-                                 end
-    | Eprim_binop Brem e1 e2 => let t1 := type_of_hfexpr e1 ce in
-                                 let t2 := type_of_hfexpr e2 ce in
-                                 match t1, t2 with
-                                 | Gtyp (Fuint w1), Gtyp (Fuint w2) => Gtyp (Fuint (minn w1 w2))
-                                 | Gtyp (Fsint w1), Gtyp (Fsint w2) => Gtyp (Fsint (minn w1 w2))
-                                 | _, _ => def_ftype
-                                 end
-    | Eprim_binop Bdshl e1 e2 => let t1 := type_of_hfexpr e1 ce in
-                                 let t2 := type_of_hfexpr e2 ce in
-                                 match t1, t2 with
-                                 | Gtyp (Fuint w1), Gtyp (Fuint w2) => Gtyp (Fuint (w1 + 2 ^ w2 - 1))
-                                 | Gtyp (Fsint w1), Gtyp (Fuint w2) => Gtyp (Fsint (w1 + 2 ^ w2 - 1))
-                                 | _, _ => def_ftype
-                                 end
-    | Eprim_binop Bdshr e1 e2 => let t1 := type_of_hfexpr e1 ce in
-                                 let t2 := type_of_hfexpr e2 ce in
-                                 match t1, t2 with
-                                 | Gtyp (Fuint w1), Gtyp (Fuint w2) => Gtyp (Fuint w1)
-                                 | Gtyp (Fsint w1), Gtyp (Fuint w2) => Gtyp (Fsint w1)
-                                 | _, _ => def_ftype
-                                 end
-    | Eprim_binop Bcat e1 e2 => let t1 := type_of_hfexpr e1 ce in
-                                let t2 := type_of_hfexpr e2 ce in
-                                match t1, t2 with
-                                | Gtyp (Fuint w1), Gtyp (Fuint w2) => Gtyp (Fuint (w1 + w2))
-                                | Gtyp (Fsint w1), Gtyp (Fsint w2) => Gtyp (Fuint (w1 + w2))
-                                | _, _ => def_ftype
-                                end
-    | Eprim_binop Band e1 e2
-    | Eprim_binop Bor e1 e2
-    | Eprim_binop Bxor e1 e2 => let t1 := type_of_hfexpr e1 ce in
-                                let t2 := type_of_hfexpr e2 ce in
-                                match t1, t2 with
-                                | Gtyp (Fuint w1), Gtyp (Fuint w2) => Gtyp (Fuint (maxn w1 w2))
-                                | Gtyp (Fsint w1), Gtyp (Fsint w2) => Gtyp (Fuint (maxn w1 w2))
-                                | _, _ => def_ftype
-                                end
-    | Emux c e1 e2 => let t1 := type_of_hfexpr e1 ce in
-                      let t2 := type_of_hfexpr e2 ce in
-                      mux_types t1 t2
-    | Evalidif c e1 => type_of_hfexpr e1 ce
-    end.
+(** Pass ExpandWhens *)
 
-
-  (********************************************************************************)
-
-  Definition is_init (s : hfstmt) : bool :=
-     match s with
-     | Spcnct _ _ | Sfcnct _ _ | Sinvalid _ | Swhen _ _ _
-     (* | Sstop _ _ _  *)| Sskip => false
-     | _ => true
-     end.
-
-   Fixpoint is_init_all_t s : bool :=
-     match (s) with
-     | nil => true
-     | cons h t => if (is_init h) then is_init_all_t t else false
-     end.
-
-   Fixpoint not_init_all s : bool :=
-     match s with
-     | nil => true
-     | cons h t => if (is_init h) then false else not_init_all t
-     end.
-
-   Parameter new_comp_name : var -> Prop.
-
-   Parameter new_v_cefind_none:
-     forall v,
-     new_comp_name v ->
-     forall ce: cenv, CE.find v ce = None.
-
-
-
-  (********************************************************************************)
-
-
-
-  Definition upd_regtyp t r :=
-    mk_hfreg t (clock r) (reset r).
-
-  Definition upd_memtyp t m :=
-    mk_hfmem t (depth m) (reader m) (writer m) (read_latency m) (write_latency m) (read_write m).
-
-  Definition is_bundle t :=
-    match t with Btyp _ => true | _ => false end.
-
-  Definition is_vector t :=
-    match t with Atyp _ _ => true | _ => false end.
-
-  Fixpoint is_deftyp t :=
-    match t with
-    | Gtyp (Fsint 0)
-    | Gtyp (Fuint 0) => true
-    | Atyp tn _ => is_deftyp tn
-    | Btyp Fnil => true
-    | Btyp bt => is_deftyp_f bt
-    | _ => false
-    end
-  with is_deftyp_f bt :=
-         match bt with
-         | Fnil => false
-         | Fflips v f tv fs => is_deftyp tv || (is_deftyp_f fs)
-         end.
-
-  (* given 2 equivalent types, return the one with larger width *)
-  Fixpoint max_width t1 t2 :=
-    match t1, t2 with
-    | Gtyp (Fsint w1), Gtyp (Fsint w2) => Gtyp (Fsint (maxn w1 w2))
-    | Gtyp (Fuint w1), Gtyp (Fuint w2) => Gtyp (Fuint (maxn w1 w2))
-    | Atyp tn1 n1, Atyp tn2 n2 => if n2 == n1 then Atyp (max_width tn1 tn2) n1
-                                  else t1
-    | Btyp bt1, Btyp bt2 => Btyp (max_width_f bt1 bt2)
-    | _, _ => t1
-    end
-  with max_width_f bt1 bt2 :=
-         match bt1, bt2 with
-         | Fflips v1 ft1 t1 fs1, Fflips v2 ft2 t2 fs2 =>
-           Fflips v1 ft1 (max_width t1 t2) (max_width_f fs1 fs2)
-         | _, _ => bt1
-         end.
-
-  Lemma max_width_ftype_equiv :
-    forall t1 t2,
-      ftype_equiv t1 t2 ->
-      ftype_equiv t1 (max_width t1 t2)
-  with max_width_ffield_equiv :
-         forall f1 f2,
-           fbtyp_equiv f1 f2 ->
-           fbtyp_equiv f1 (max_width_f f1 f2).
-  Proof.
-    elim.
-    - move => f . elim; try discriminate.
-      elim f;
-       try (intro; elim; try done).
-    - move => t1 Hm n.
-      elim; try done. move => t2 Hn n2.
-      move => Heqt; rewrite /= in Heqt.
-      move : Heqt =>/andP[Hteq Heq12].
-      rewrite (eqP Hteq) /= !eq_refl andTb.
-      by apply Hm.
-    - move => f1. elim; try discriminate.
-      move => f2. apply max_width_ffield_equiv.
-    elim.
-    - elim; try done.
-    - move => v1 fp1 t1 ff1 Hm.
-      elim. case fp1 => //.
-      move => v2 fp2 t2 ff2 Hn.
-      case fp1; case fp2; try discriminate.
-      + move =>/= /andP[/andP [Heq1 Heq2] Heq3].
-        rewrite eq_refl andTb.
-        apply /andP; split.
-        * apply max_width_ftype_equiv; done.
-        * apply Hm; done.
-      + move =>/= /andP[/andP [Heq1 Heq2] Heq3].
-        rewrite eq_refl andTb.
-        apply /andP; split.
-        * apply max_width_ftype_equiv; done.
-        * apply Hm; done.
-  Qed.
-
-  (* directly upd a field of a ftype with name 'v' with given type t, the field width upd to larger one *)
-  (* if it has no such field, return itself *)
-  Fixpoint upd_name_ftype ft v t : ftype :=
-    match ft with
-    | Gtyp gt => t
-    | Atyp tn n => Atyp (upd_name_ftype tn v t) n
-    | Btyp bt => Btyp (upd_name_ffield bt v t)
-    end
-  with upd_name_ffield bt v t : ffield :=
-         match bt with
-         | Fnil => Fnil
-         | Fflips v1 fp t1 fs => if v1 == v then Fflips v1 fp (max_width t1 t) fs
-                                 else Fflips v1 fp (upd_name_ftype t1 v t)
-                                             (upd_name_ffield fs v t)
-         end.
-
-  Lemma upd_type_equiv :
-    forall t r v ce, ~~ is_deftyp (type_of_hfexpr (eref (esubfield r v)) ce) ->
-                     ftype_equiv (type_of_hfexpr (eref (esubfield r v)) ce) t ->
-                     ftype_equiv (base_type_of_ref r ce)
-                                 (upd_name_ftype (base_type_of_ref r ce) (v2var v) t).
-  Proof.
-  Admitted.
-
-  Fixpoint upd_vectyp vt t : ftype :=
-    match vt with
-    | Gtyp gt => t
-    | Atyp tn n => Atyp (upd_vectyp tn t) n
-    | Btyp bt => Btyp bt
-    end.
-
-  Lemma upd_vectyp_equiv :
-    forall t r n ce, ftype_equiv (type_of_hfexpr (eref (esubaccess r n)) ce) t ->
-                     ftype_equiv (base_type_of_ref r ce)
-                                 (upd_vectyp (base_type_of_ref r ce) t).
-  Proof.
-  Admitted.
-
-  Fixpoint typeConstraints (f1 f2 : nat -> nat -> bool) (t1 t2 : ftype) : bool :=
-    match t1, t2 with
-    | Gtyp (Fuint w1), Gtyp (Fuint w2)
-    | Gtyp (Fsint w1), Gtyp (Fsint w2) => f1 w1 w2
-    | Gtyp Fclock, Gtyp Fclock => true
-    | Atyp t1 n1, Atyp t2 n2 => (n1 == n2) && typeConstraints f1 f2 t1 t2
-    | Btyp b1, Btyp b2 => typeConstraints_f f1 f2 b1 b2
-    | _, _ => false
-    end
-  with typeConstraints_f f1 f2 b1 b2 :=
-         match b1, b2 with
-         | Fnil, Fnil => true
-         | Fflips v1 Flipped t1 fs1, Fflips v2 Flipped t2 fs2 =>
-           (v1 == v2) && (typeConstraints f2 f1 t1 t2) && typeConstraints_f f1 f2 fs1 fs2
-         | Fflips v1 Nflip t1 fs1, Fflips v2 Nflip t2 fs2 =>
-           (v1 == v2) && typeConstraints f1 f2 t1 t2 && typeConstraints_f f1 f2 fs1 fs2
-         | _, _ => false
-         end.
-
-
-
-  (* type constraint : dst type ge than src *)
-  Definition typeConstraintsGe t1 t2 := typeConstraints geq ltn t1 t2.
-
-  (* type constraint exclude default type *)
-  Definition typeConstraintsGe_exdef t1 t2 :=
-    if is_deftyp t1 then true
-    else typeConstraintsGe t1 t2.
-
-  (********************************************************************************)
-
-  (** Pass ResolveFlow *)
-  (* rhs passive type ? TBD. *)
-
-  (* Fixpoint resolveFlow_fun st te : bool := *)
-  (*   match st with *)
-  (*   | Sfcnct r e => *)
-  (*     ftype_equiv (type_of_ref r te) (type_of_hfexpr e te) && valid_rhs_fexpr e te *)
-  (*     && (valid_lhs_orient (orient_of_comp (snd (CE.vtyp (base_ref r) te)))) *)
-  (*   | Spcnct r e => *)
-  (*     ftype_weak_equiv (type_of_ref r te) (type_of_hfexpr e te) && valid_rhs_fexpr e te *)
-  (*     && (valid_lhs_orient (orient_of_comp (snd (CE.vtyp (base_ref r) te)))) *)
-  (*   | Sinvalid e => valid_rhs_ref e te *)
-  (*   | Sreg r rt => match (reset rt) with *)
-  (*                  | NRst => true *)
-  (*                  | Rst r1 r2 => valid_rhs_fexpr r2 te *)
-  (*                  end *)
-  (*   | _ => true *)
-  (*   end. *)
-
-  (********************************************************************************)
-
-   (** Pass ExpandWhens *)
-(* COMMENT OUT START HERE *)
-(*
-  
-   (* The pass translates a FIRRTL statement sequence (but one without aggregate types/aggregate connects)
-      to one where when statements are replaced by suitable multiplexers or validifs.
-      It also handles the last connect semantics. *)
+(* The pass translates a FIRRTL statement sequence (but one without aggregate types/aggregate connects)
+   to one where when statements are replaced by suitable multiplexers or validifs.
+   It also handles the last connect semantics. *)
 
    (* a type to indicate connects *)
    Inductive def_expr : Type :=
@@ -1658,40 +168,42 @@ Proof.
           CE.map2 (map2_helper_cs_tf c) (snd true_branch) (snd false_branch))
    .
 
-   Definition option_and (simcond : option hfexpr) (cond : hfexpr) : hfexpr :=
-   (* calculates the conjunction between two conditions if present *)
+   (* Definition option_and (simcond : option hfexpr) (cond : hfexpr) : hfexpr :=
+   (* calculates the conjunction between two conditions if present.
+      This function is only used if there are simulation statements like Sstop. *)
    match simcond with
    | None => cond
    | Some s => eprim_binop Band s cond
-   end.
+   end. *)
 
    (* Because nat and ftype are not mutually recursive types we cannot define a mutually recursive
       initialization function for registers including array types.
       Therefore we construct, in a mutual recursion, a function that initializes one element of the array.
       After that we call the constructed function for every element of the array. *)
 
-   Fixpoint init_register_vector (v : nat -> href) (array_size : nat) (type : ftype) (ce : cenv) : (nat -> cmap -> cmap) * nat :=
+   Fixpoint init_register_vector (v : nat -> href) (array_size : nat) (type : ftype) : (nat -> cmap -> cmap) * nat :=
    (* Produces a function that initializes v to itself.
-      Input:  * v = href of the variable that needs to be initialized (possibly this is already an array)
+      Input:  * v = href of the variable that needs to be initialized
+                    (possibly this is already an array, that's why it is a function from nat to href)
               * array_size = size of the array v (if it's not an array, array_size == 1)
               * type = type of (a single element of the array) v <number>
               * ce = component environment
       Output: * nat -> cmap -> cmap : a function that initializes one element of the array (by modifying a cmap accordingly)
               * nat : size of the array *)
    match type with
-   | Gtyp _ => ((fun n : nat => CE.add (expand_eref (v n) ce) (D_fexpr (Eref (v n)))), array_size)
-   | Atyp el_type n => init_register_vector (fun m : nat => Esubindex (v (m / array_size)) (m mod array_size)) (array_size * n) el_type ce
-   | Btyp ff => init_register_bundle v array_size ff ce
+   | Gtyp _ => ((fun n : nat => CE.add (ref2var (v n)) (D_fexpr (Eref (v n)))), array_size)
+   | Atyp el_type n => init_register_vector (fun m : nat => Esubindex (v (m / array_size)) (m mod array_size)) (array_size * n) el_type
+   | Btyp ff => init_register_bundle v array_size ff
    end
-   with init_register_bundle (v : nat -> href) (array_size : nat) (ff : ffield) (ce : cenv) : (nat -> cmap -> cmap) * nat :=
+   with init_register_bundle (v : nat -> href) (array_size : nat) (ff : ffield) : (nat -> cmap -> cmap) * nat :=
    match ff with
    | Fnil => ((fun (n : nat) (cm : cmap) => cm), 0)
    | Fflips field_name Nflip field_type ff_tail =>
-        let init_field := init_register_vector (fun n : nat => Esubfield (v n) (var2v field_name)) array_size field_type ce in
-        let init_tail := init_register_bundle v array_size ff_tail ce in
-        ((fun n : nat => if n < snd init_field then fst init_field n
-                                               else fst init_tail (n - snd init_field)),
-         snd init_field + snd init_tail)
+        let init_field := init_register_vector (fun n : nat => Esubfield (v n) field_name) array_size field_type
+        in let init_tail := init_register_bundle v array_size ff_tail
+           in ((fun n : nat => if n <? snd init_field then fst init_field n
+                                                      else fst init_tail (n - snd init_field)),
+               snd init_field + snd init_tail)
    | Fflips _ Flipped _ _ => (* error: a register must have a passive type *) ((fun (n : nat) (cm : cmap) => empty_cmap), 0)
    end.
 
@@ -1703,33 +215,33 @@ Proof.
    | S m => init_apply_initializer fn m (fn m cm)
    end.
 
-   Definition init_register (id : V.T) (type : ftype) (ce : cenv) (cm : cmap) : cmap :=
+   Definition init_register (id : VarOrder.T) (type : ftype) (cm : cmap) : cmap :=
    (* Initializes the register id, which is of type type. *)
-   let initializer := init_register_vector (fun n : nat => Eid id) 1 type ce in
-   init_apply_initializer (fst initializer) (snd initializer) cm.
+   let initializer := init_register_vector (fun n : nat => Eid id) 1 type
+   in init_apply_initializer (fst initializer) (snd initializer) cm.
 
    (* Identifiers for the fields of a memory port *)
-   Parameter mem_port_addr : V.T.
-   Parameter mem_port_en : V.T.
-   Parameter mem_port_clk : V.T.
-   Parameter mem_port_data : V.T.
-   Parameter mem_port_mask : V.T.
+   Parameter mem_port_addr : VarOrder.T.
+   Parameter mem_port_en : VarOrder.T.
+   Parameter mem_port_clk : VarOrder.T.
+   Parameter mem_port_data : VarOrder.T.
+   Parameter mem_port_mask : VarOrder.T.
 
-   Fixpoint init_memory_reader (id : V.T) (reader : seq V.T) (ce : cenv) (cm : cmap) : cmap :=
+   Fixpoint init_memory_reader (id : VarOrder.T) (reader : seq VarOrder.T) (cm : cmap) : cmap :=
    (* Helper function for init_memory. It initializes the read ports that are indicated in reader. *)
    match reader with
    | [::] => cm
-   | r :: rtail => init_memory_reader id rtail ce
-                   (CE.add (expand_eref (Esubfield (Esubfield (Eid id) r) mem_port_addr) ce) D_undefined
-                      (CE.add (expand_eref (Esubfield (Esubfield (Eid id) r) mem_port_en) ce) D_undefined
-                         (CE.add (expand_eref (Esubfield (Esubfield (Eid id) r) mem_port_clk) ce) D_undefined
+   | r :: rtail => init_memory_reader id rtail
+                   (CE.add (ref2var (Esubfield (Esubfield (Eid id) r) mem_port_addr)) D_undefined
+                      (CE.add (ref2var (Esubfield (Esubfield (Eid id) r) mem_port_en)) D_undefined
+                         (CE.add (ref2var (Esubfield (Esubfield (Eid id) r) mem_port_clk)) D_undefined
                             cm
                          )
                       )
                    )
    end.
 
-   Fixpoint init_undefined_vector (v : nat -> href) (array_size : nat) (type : ftype) (value : def_expr) (ce : cenv) : (nat -> cmap -> cmap) * nat :=
+   Fixpoint init_undefined_vector (v : nat -> href) (array_size : nat) (type : ftype) (value : def_expr) : (nat -> cmap -> cmap) * nat :=
    (* Produces a function that initializes v to value (mostly D_undefined or D_invalidated).
       It can be used to initialize memory write ports (data and mask fields) and wires.
       Memory ports have to be passive, but wires allow flipped fields,
@@ -1737,78 +249,77 @@ Proof.
       Input:  * v = href of the variable that needs to be initialized (possibly this is already an array)
               * array_size = size of the array v (if it's not an array, array_size == 1)
               * type = type of v <number>
-              * ce = component environment
       Output: * nat -> cmap -> cmap : a function that initializes one element of the array (by modifying a cmap accordingly)
               * nat : size of the array *)
    match type with
-   | Gtyp _ => ((fun n : nat => CE.add (expand_eref (v n) ce) value), array_size)
-   | Atyp el_type n => init_undefined_vector (fun m : nat => Esubindex (v (m / array_size)) (m mod array_size)) (array_size * n) el_type value ce
-   | Btyp ff => init_undefined_bundle v array_size ff value ce
+   | Gtyp _ => ((fun n : nat => CE.add (ref2var (v n)) value), array_size)
+   | Atyp el_type n => init_undefined_vector (fun m : nat => Esubindex (v (m / array_size)) (m mod array_size)) (array_size * n) el_type value
+   | Btyp ff => init_undefined_bundle v array_size ff value
    end
-   with init_undefined_bundle (v : nat -> href) (array_size : nat) (ff : ffield) (value : def_expr) (ce : cenv) : (nat -> cmap -> cmap) * nat :=
+   with init_undefined_bundle (v : nat -> href) (array_size : nat) (ff : ffield) (value : def_expr) : (nat -> cmap -> cmap) * nat :=
    match ff with
    | Fnil => ((fun (n : nat) (cm : cmap) => cm), 0)
    | Fflips field_name fflip field_type ff_tail =>
-        let init_field := match fflip with Nflip => init_undefined_vector  (fun n : nat => Esubfield (v n) (var2v field_name)) array_size field_type value ce
-                                       | Flipped => init_undefined_flipped (fun n : nat => Esubfield (v n) (var2v field_name)) array_size field_type value ce
-                          end in
-        let init_tail := init_undefined_bundle v array_size ff_tail value ce in
-        ((fun n : nat => if n < snd init_field then fst init_field n
-                                               else fst init_tail (n - snd init_field)),
-         snd init_field + snd init_tail)
+        let init_field := match fflip with Nflip => init_undefined_vector  (fun n : nat => Esubfield (v n) field_name) array_size field_type value
+                                       | Flipped => init_undefined_flipped (fun n : nat => Esubfield (v n) field_name) array_size field_type value
+                          end
+        in let init_tail := init_undefined_bundle v array_size ff_tail value
+           in ((fun n : nat => if n <? snd init_field then fst init_field n
+                                                      else fst init_tail (n - snd init_field)),
+               snd init_field + snd init_tail)
    end
-   with init_undefined_flipped (v : nat -> href) (array_size : nat) (type : ftype) (value : def_expr) (ce : cenv) : (nat -> cmap -> cmap) * nat :=
+   with init_undefined_flipped (v : nat -> href) (array_size : nat) (type : ftype) (value : def_expr) : (nat -> cmap -> cmap) * nat :=
    match type with
    | Gtyp _ => ((fun (n : nat) (cm: cmap) => cm), 0)
-   | Atyp el_type n => init_undefined_flipped (fun m : nat => Esubindex (v (m / array_size)) (m mod array_size)) (array_size * n) el_type value ce
-   | Btyp ff => init_undefined_flipped_bundle v array_size ff value ce
+   | Atyp el_type n => init_undefined_flipped (fun m : nat => Esubindex (v (m / array_size)) (m mod array_size)) (array_size * n) el_type value
+   | Btyp ff => init_undefined_flipped_bundle v array_size ff value
    end
-   with init_undefined_flipped_bundle (v : nat -> href) (array_size : nat) (ff : ffield) (value : def_expr) (ce : cenv) : (nat -> cmap -> cmap) * nat :=
+   with init_undefined_flipped_bundle (v : nat -> href) (array_size : nat) (ff : ffield) (value : def_expr) : (nat -> cmap -> cmap) * nat :=
    match ff with
    | Fnil => ((fun (n : nat) (cm : cmap) => cm), 0)
    | Fflips field_name fflip field_type ff_tail =>
-        let init_field := match fflip with Nflip => init_undefined_flipped (fun n : nat => Esubfield (v n) (var2v field_name)) array_size field_type value ce
-                                       | Flipped => init_undefined_vector  (fun n : nat => Esubfield (v n) (var2v field_name)) array_size field_type value ce
-                          end in
-        let init_tail := init_undefined_flipped_bundle v array_size ff_tail value ce in
-        ((fun n : nat => if n < snd init_field then fst init_field n
-                                               else fst init_tail (n - snd init_field)),
-         snd init_field + snd init_tail)
+        let init_field := match fflip with Nflip => init_undefined_flipped (fun n : nat => Esubfield (v n) field_name) array_size field_type value
+                                       | Flipped => init_undefined_vector  (fun n : nat => Esubfield (v n) field_name) array_size field_type value
+                          end
+        in let init_tail := init_undefined_flipped_bundle v array_size ff_tail value
+           in ((fun n : nat => if n <? snd init_field then fst init_field n
+                                                      else fst init_tail (n - snd init_field)),
+               snd init_field + snd init_tail)
    end.
 
-   Fixpoint init_memory_writer (id : V.T) (data_type : ftype) (writer : seq V.T) (ce : cenv) (cm : cmap) : cmap :=
+   Fixpoint init_memory_writer (id : VarOrder.T) (data_type : ftype) (writer : seq VarOrder.T) (cm : cmap) : cmap :=
    (* Helper function for init_memory. It initializes the write ports that are indicated in writer. *)
    match writer with
    | [::] => cm
-   | w :: wtail => let initializer_data := init_undefined_vector (fun n : nat => (Esubfield (Esubfield (Eid id) w) mem_port_data)) 1 data_type D_undefined ce in
-                   let initializer_mask := init_undefined_vector (fun n : nat => (Esubfield (Esubfield (Eid id) w) mem_port_mask)) 1 data_type D_undefined ce in
-                   init_memory_writer id data_type wtail ce
-                   (CE.add (expand_eref (Esubfield (Esubfield (Eid id) w) mem_port_addr) ce) D_undefined
-                      (CE.add (expand_eref (Esubfield (Esubfield (Eid id) w) mem_port_en) ce) D_undefined
-                         (CE.add (expand_eref (Esubfield (Esubfield (Eid id) w) mem_port_clk) ce) D_undefined
-                            (init_apply_initializer (fst initializer_data) (snd initializer_data)
-                               (init_apply_initializer (fst initializer_mask) (snd initializer_mask) cm)
+   | w :: wtail => let initializer_data := init_undefined_vector (fun n : nat => (Esubfield (Esubfield (Eid id) w) mem_port_data)) 1 data_type D_undefined
+                   in let initializer_mask := init_undefined_vector (fun n : nat => (Esubfield (Esubfield (Eid id) w) mem_port_mask)) 1 data_type D_undefined
+                      in init_memory_writer id data_type wtail
+                         (CE.add (ref2var (Esubfield (Esubfield (Eid id) w) mem_port_addr)) D_undefined
+                            (CE.add (ref2var (Esubfield (Esubfield (Eid id) w) mem_port_en)) D_undefined
+                               (CE.add (ref2var (Esubfield (Esubfield (Eid id) w) mem_port_clk)) D_undefined
+                                  (init_apply_initializer (fst initializer_data) (snd initializer_data)
+                                     (init_apply_initializer (fst initializer_mask) (snd initializer_mask) cm)
+                                  )
+                               )
                             )
                          )
-                      )
-                   )
    end.
 
-   Fixpoint memport_ids (m : seq mem_port) : seq V.T :=
+   Fixpoint memport_ids (m : seq mem_port) : seq VarOrder.T :=
      match m with
-     | nil => nil
-     | cons pid pids => cons (id pid) (memport_ids pids)
+     | [::] => [::]
+     | pid :: pids => (id pid) :: (memport_ids pids)
      end.
-   
-   Definition init_memory (id : V.T) (m : hfmem) (ce : cenv) (cm : cmap) : cmap :=
+
+   Definition init_memory (id : VarOrder.T) (m : hfmem) (cm : cmap) : cmap :=
    (* This helper function initializes a memory named v with description m.
       In particular, all reader and writer ports are declared undefined. *)
-   init_memory_writer id (data_type m) (memport_ids (writer m)) ce (init_memory_reader id (memport_ids (reader m)) ce cm).
+   init_memory_writer id (data_type m) (memport_ids (writer m)) (init_memory_reader id (memport_ids (reader m)) cm).
 
-   Definition init_wire (id : V.T) (type : ftype) (ce : cenv) (cm : cmap) : cmap :=
+   Definition init_wire (id : VarOrder.T) (type : ftype) (cm : cmap) : cmap :=
    (* Initializes a wire named id with type type. *)
-   let initializer := init_undefined_vector (fun n : nat => (Eid id)) 1 type D_undefined ce in
-   init_apply_initializer (fst initializer) (snd initializer) cm.
+   let initializer := init_undefined_vector (fun n : nat => (Eid id)) 1 type D_undefined
+   in init_apply_initializer (fst initializer) (snd initializer) cm.
 
 (* Inductive error_type (T : Type) : Type :=
    | ECorrect : T -> error_type
@@ -1818,43 +329,39 @@ Proof.
    | Einternal (* e.g. if a pass receives input that should have been handled by earlier passes *)
    | E...
 
-   Definition init_wire (id : V.T) (type : ftype) (ce : cenv) (cm : cmap) : error_type cmap :=
+   Definition init_wire (id : VarOrder.T) (type : ftype) (ce : CE.env) (cm : cmap) : error_type cmap :=
    (* Initializes a wire named id with type type. May return an error message. *)
    match init_undefined_vector (fun n : nat => (Eid id)) 1 type D_undefined ce with
    Some initializer => init_apply_initializer (fst initializer) (snd initializer) cm
    error => error
    end. *)
 
-   Definition init_instance (id: V.T) (mdl: V.T) (ce : cenv) (cm : cmap) : cmap :=
+   Definition init_instance (id: VarOrder.T) (mdl: VarOrder.T) (ce : CE.env) (cm : cmap) : cmap :=
    (* This function should initialize the ports that connect the current module with module mdl under the name id,
       which is instantiated here.
       It is assumed that the type of the module is stored in ce already. *)
-   let initializer := init_undefined_flipped (fun n : nat => (Eid id)) 1 (type_of_cmpnttyp (fst (CE.vtyp mdl ce))) D_undefined ce in
-   init_apply_initializer (fst initializer) (snd initializer) cm.
+   let initializer := init_undefined_flipped (fun n : nat => Eid id) 1 (type_of_cmpnttyp (fst (CE.vtyp mdl ce))) D_undefined
+   in init_apply_initializer (fst initializer) (snd initializer) cm.
 
-   Definition invalidate_cmpnt (ref : href) (ce : cenv) (cm : cmap) : cmap :=
+   Definition invalidate_cmpnt (ref : href) (cm : cmap) : cmap :=
    (* Sets the component ref to invalid, to indicate that the programmer let it unconnected on purpose. *)
-   (* If "is invalid" statements are expanded by ExpandConnects, then it would suffice to return
-      CE.add (expand_eref ref ce) D_invalidated cm. *)
-   let initializer := init_undefined_vector (fun n : nat => ref) 1 (type_of_ref ref ce) D_invalidated ce in
-   init_apply_initializer (fst initializer) (snd initializer) cm.
+      CE.add (ref2var ref) D_invalidated cm.
+   (*let initializer := init_undefined_vector (fun n : nat => ref) 1 (type_of_ref ref ce) D_invalidated ce in
+   init_apply_initializer (fst initializer) (snd initializer) cm.*)
 
-   Fixpoint expandBranch_fun (ss : hfstmt_seq) (ce : cenv) (cm : cmap) (simcond : option hfexpr) : (hfstmt_seq * cmap) :=
+   Fixpoint expandBranch_fun (ss : hfstmt_seq) (ce : CE.env) (cm : cmap) : (hfstmt_seq * cmap) :=
    (* This is the main function of ExpandWhens. It replaces when statements by expressions containing
       multiplexers/validifs where necessary.  It has the following interface:
       Input:  * ss = sequence of statements that are a final fragment of a module definition
                 or a final fragment of a branch
-                (not containing partial or aggregate connects or aggregate "is invalid" statements;
+                (not containing partial or aggregate connects;
                 possibly containing repeated connects and when statements)
-              * ce = component environment, containing the type declarations
-                of the module (this has been found in earlier passes and is not updated)
+              * ce = component environment, containing the port declarations of other modules
+                (this has been found in earlier passes and is not updated)
               * cm = map of connections that have been defined in the previous statements of the module definition
                 (including, when applicable, in the previous statements of the branch).
                 This map is used in case a when statement only replaces a connect in one branch;
                 in that case, the other branch has to copy the connect from this map.
-              * simcond = condition of the outer when statement;
-                this is used to constrain simulation statement Sstop
-                in case it appears within a when statement.
       Output: a pair consisting of
               * sequence of statements, mainly containing declarations of registers and wires,
                 that should become part of the resulting code (because registers and wires etc.
@@ -1864,47 +371,52 @@ Proof.
    match ss with
    | Qnil => (qnil, cm)
    | Qcons s ss_tail => match s with
-                 | @Sskip _ => expandBranch_fun ss_tail ce cm simcond (* no translation needed *)
-                 | @Swire _ id type => let result := expandBranch_fun ss_tail ce (init_wire id type ce cm) simcond in
-                                       (Qcons s (fst result), snd result)
-                 | @Sreg _ id reg => let result := expandBranch_fun ss_tail ce (init_register id (type reg) ce cm) simcond in
-                                     (Qcons s (fst result), snd result)
-                 | @Smem _ id mem => let result := expandBranch_fun ss_tail ce (init_memory id mem ce cm) simcond in
-                                     (Qcons s (fst result), snd result)
-                 | @Sinst _ id mdl => let result := expandBranch_fun ss_tail ce (init_instance id mdl ce cm) simcond in
-                                   (Qcons s (fst result), snd result)
-                 | @Snode _ _ _ => let result := expandBranch_fun ss_tail ce cm simcond in
-                                   (Qcons s (fst result), snd result)
-                 | @Sfcnct _ ref expr => expandBranch_fun ss_tail ce (CE.add (expand_eref ref ce) (D_fexpr expr) cm) simcond
-                 | @Spcnct _ _ _ => (* error: should have been expanded earlier *) (qnil, empty_cmap)
-                 | @Sinvalid _ ref => expandBranch_fun ss_tail ce (invalidate_cmpnt ref ce cm) simcond
-                 | @Swhen _ cond ss_true ss_false => let combined_branches := combine_branches cond (expandBranch_fun ss_true  ce cm (Some (option_and simcond cond)))
-                                                                                                    (expandBranch_fun ss_false ce cm (Some (option_and simcond (eprim_unop Unot cond)))) in
-                                         let result := expandBranch_fun ss_tail ce (snd combined_branches) simcond in
-                                         (Qcat (fst combined_branches) (fst result), snd result)
-                 (* | @Sstop _ clk cond exit => let result := expandBranch_fun ss_tail ce cm simcond in *)
-                 (*                             (Qcons (Sstop clk (option_and simcond cond) exit) (fst result), snd result) *)
-                 end
+                        | @Sskip _ => expandBranch_fun ss_tail ce cm (* no translation needed *)
+                        | @Swire _ id type => let result := expandBranch_fun ss_tail ce (init_wire id type cm)
+                                              in (Qcons s (fst result), snd result)
+                        | @Sreg _ id reg => let result := expandBranch_fun ss_tail ce (init_register id (type reg) cm)
+                                            in (Qcons s (fst result), snd result)
+                        | @Smem _ id mem => let result := expandBranch_fun ss_tail ce (init_memory id mem cm)
+                                            in (Qcons s (fst result), snd result)
+                        | @Sinst _ id mdl => let result := expandBranch_fun ss_tail ce (init_instance id mdl ce cm)
+                                             in (Qcons s (fst result), snd result)
+                        | @Snode _ _ _ => let result := expandBranch_fun ss_tail ce cm
+                                          in (Qcons s (fst result), snd result)
+                        | @Sfcnct _ ref expr => expandBranch_fun ss_tail ce (CE.add (ref2var ref) (D_fexpr expr) cm)
+                        | @Spcnct _ _ _ => (* error: should have been expanded earlier *) (qnil, empty_cmap)
+                        | @Sinvalid _ ref => expandBranch_fun ss_tail ce (invalidate_cmpnt ref cm)
+                        | @Swhen _ cond ss_true ss_false => let combined_branches := combine_branches cond (expandBranch_fun ss_true  ce cm)
+                                                                                                           (expandBranch_fun ss_false ce cm)
+                                                            in let result := expandBranch_fun ss_tail ce (snd combined_branches)
+                                                               in (Qcat (fst combined_branches) (fst result), snd result)
+                        (* | @Sstop _ clk cond exit => let result := expandBranch_fun ss_tail ce cm simcond *)
+                        (*                             in (Qcons (Sstop clk (option_and simcond cond) exit) (fst result), snd result) *)
+                        end
    end.
 
-   Fixpoint init_ports (ports : seq hfport) (ce : cenv) (cm : cmap) : cmap :=
+   Fixpoint init_ports (ports : seq hfport) (cm : cmap) : cmap :=
    (* This helper function sets the ports of a module to undefined. *)
    match ports with
    | [::] => cm
-   | Finput  id type :: ports_tail => let initializer := init_undefined_flipped (fun n : nat => Eid id) 1 type D_undefined ce in
-                                      init_ports ports_tail ce (init_apply_initializer (fst initializer) (snd initializer) cm)
-   | Foutput id type :: ports_tail => let initializer := init_undefined_vector  (fun n : nat => Eid id) 1 type D_undefined ce in
-                                      init_ports ports_tail ce (init_apply_initializer (fst initializer) (snd initializer) cm)
+   | Finput  id type :: ports_tail => let initializer := init_undefined_flipped (fun n : nat => Eid id) 1 type D_undefined
+                                      in init_ports ports_tail (init_apply_initializer (fst initializer) (snd initializer) cm)
+   | Foutput id type :: ports_tail => let initializer := init_undefined_vector  (fun n : nat => Eid id) 1 type D_undefined
+                                      in init_ports ports_tail (init_apply_initializer (fst initializer) (snd initializer) cm)
    end.
 
-   Definition recode_cmap_entry (id : V.T) (dexpr : def_expr) (ss : hfstmt_seq) : hfstmt_seq :=
+   Definition recode_cmap_entry (id : VarOrder.T) (dexpr : def_expr) (ss : hfstmt_seq) : hfstmt_seq :=
    (* This helper function for recode_map translates one entry of the cmap into a statement
       that is added to the statement sequence ss. *)
    match dexpr with
    | D_undefined => ss (* the user has erroneously not connected to id *)
-   | D_invalidated => Qcons (sinvalid (Eid id)) ss (* the user has given an "is invalid" statement. Copy it. *)
-   | D_fexpr expr => Qcons (sfcnct (Eid id) expr) ss
-   (* instead of Eid id, we should generate the appropriate (possibly structured) href above. *)
+   | D_invalidated => match var2ref id with
+                      | None => (* error *) qnil
+                      | Some ref => Qcons (sinvalid ref) ss (* the user has given an "is invalid" statement. Copy it. *)
+                      end
+   | D_fexpr expr => match var2ref id with
+                     | None => (* error *) qnil
+                     | Some ref => Qcons (sfcnct ref expr) ss
+                     end
    end.
 
    Definition recode_cmap (cm : cmap) : hfstmt_seq :=
@@ -1925,7 +437,7 @@ Proof.
    so they could be placed at the end of the module, in the same order as they appear in
    the original.  But registers cannot be handled that easily.)
 
-   Fixpoint dependencies_present (expr : hfexpr) (ce : cenv) (cm : cmap) : bool :=
+   Fixpoint dependencies_present (expr : hfexpr) (ce : CE.env) (cm : cmap) : bool :=
    (* Returns true iff expr contains a non-register component that is present in cm.
       (Dependencies on registers can be disregarded because one always reads the old value
       and writes the new value to a register.) *)
@@ -1938,7 +450,7 @@ Proof.
    | Emux expr0 expr1 expr2 => dependencies_present expr0 cm || dependencies_present expr1 cm || dependencies_present expr2 cm
    | Eref ref => dependencies_present_ref ref cm
    end
-   with dependencies_present_ref (ref : href) (ce : cenv) (cm : cmap) : bool :=
+   with dependencies_present_ref (ref : href) (ce : CE.env) (cm : cmap) : bool :=
    match ref with
    | Eid id => match find id ce with
                | None (* error: undeclared identifier used *)
@@ -1950,7 +462,7 @@ Proof.
    | Esubaccess ref expr => dependencies_present_ref ref cm || dependencies_present expr cm
    end.
 
-   Definition recode_cmap_sorted_entry (ce : cenv) (id : V.T) (dexpr : def_expr) (ss_cm : hfstmt_seq * cmap) : hfstmt_seq * cmap :=
+   Definition recode_cmap_sorted_entry (ce : CE.env) (id : VarOrder.T) (dexpr : def_expr) (ss_cm : hfstmt_seq * cmap) : hfstmt_seq * cmap :=
    (* This helper function for recode_map_sorted translates one entry of the cmap into a statement
       that is added to the statement sequence ss. However, the current entry is only added if all
       its dependencies have been handled earlier. To this end, snd ss_cm is the map without the
@@ -1962,9 +474,9 @@ Proof.
                      else (Qcons (sfcnct (Eid id) expr) (fst ss_cm), remove id (snd ss_cm))
    end.
 
-   Function recode_cmap_sorted (ce : cenv) (cm : cmap) (ss : hfstmt_seq)
-   (cm_is_well_founded : forall cm' : cmap, (forall (id : V.T) (dexpr : def_expr), CE.MapsTo id dexpr cm' -> CE.MapsTo id dexpr cm) ->
-                                exists (id : V.T) (dexpr : def_expr),
+   Function recode_cmap_sorted (ce : CE.env) (cm : cmap) (ss : hfstmt_seq)
+   (cm_is_well_founded : forall cm' : cmap, (forall (id : VarOrder.T) (dexpr : def_expr), CE.MapsTo id dexpr cm' -> CE.MapsTo id dexpr cm) ->
+                                exists (id : VarOrder.T) (dexpr : def_expr),
                                        CE.MapsTo id dexpr cm' /\
                                        (dexpr = D_undefined \/
                                         dexpr = D_invalidated \/
@@ -1976,36 +488,71 @@ Proof.
       The last parameter is a proof that this is the case.  Based on that parameter, one can prove the
       obligations that come with { measure cardinal cm }. *)
    if CE.empty cm then ss
-   else let result := CE.fold (recode_cmap_sorted_entry ce) cm (ss, FSet.empty) in
-        recode_cmap_sorted (snd result) (fst result) cm_is_well_founded. *)
+   else let result := CE.fold (recode_cmap_sorted_entry ce) cm (ss, FSet.empty)
+        in recode_cmap_sorted (snd result) (fst result) cm_is_well_founded. *)
 
    (* Perhaps a better way is to construct a dag.  The dag implicitly contains the proof
       that there are no cycles.  That reminds me: there are already some graph functions
       in some Coq library; in particular, the function to calculate sccs can be used for
       this end. *)
 
-   Definition expandWhen_fun (mdl : hfmodule) (ce : cenv) : hfmodule :=
+   Definition expandWhen_fun (mdl : hfmodule) (ce : CE.env) : hfmodule :=
    (* This function provides an interface to the main function.
       Input:  * mdl = module definition
                 (its statements do not contain partial or aggregate connects;
                 they may contain double connects and when statements)
-              * ce = component environment, containing the type declarations
-                of the module and the interface declarations of all other modules
+              * ce = component environment, containing the interface declarations of all other modules
                 (this has been found in earlier passes and is not updated)
       Output: translated statement sequence of the module *)
    match mdl with
-   | FInmod id ports ss => let result := expandBranch_fun ss ce (init_ports ports ce empty_cmap) None in
-                           FInmod id ports (Qcat (fst result) (recode_cmap (snd result)))
-   | FExmod _ _ ss => (* error: external modules cannot be handled for verification *) mdl
+   | FInmod id ports ss => let result := expandBranch_fun ss ce (init_ports ports empty_cmap)
+                           in FInmod id ports (Qcat (fst result) (recode_cmap (snd result)))
+   | FExmod _ _ _ => (* error: external modules cannot be handled for verification *) mdl
    end.
 
-   (* This data type is meant to describe the resulting value of a component depending on the execution path.
+   (* Specification of the semantics.
+      The semantics of when statements and last connect is:
+
+      +------------------------------------------------------------------------+
+      | For every (ground-type) sink element, ExpandWhens produces the connect |
+      | (= Sfcnct or Sinvalid) that appears last on any execution path through |
+      | the module.  If there are multiple execution paths where the component |
+      | containing this sink element is declared, ExpandWhens seleects between |
+      | them using a multiplexer or validif expression.                        |
+      | (If there is some execution path where the sink element is declared    |
+      | but is neither declared invalid [Sinvalid] not connected [Sfcnct], the |
+      | program is erroneous; in that case, ExpandWhens does not produce any   |
+      | connect for this sink element.)                                        |
+      +------------------------------------------------------------------------+
+
+      To simplify matters, we mainly concentrate on the correctness of expandBranch_fun,
+      i.e., we specify that the correct cmap is created (which will be translated to
+      the correct sequence of connect statements by recode_cmap).
+      The principle is this:
+      1. A type expr_tree models the different connects that may appear on different
+         execution paths.
+      2. Function expandBranch_one_var_sem constructs an expr_tree for one ground-type
+         element.
+      3. Function expr_tree_to_def_expr translates this expr_tree to a def_expr
+         (i.e. an entry in cmap).
+         This corresponds to the semantics for a single ground-type element.
+
+      4. Function expandBranch_one_component_sem_conform checks for every ground element
+         of one component whether a cmap (typically, the return value of expandBranch_fun)
+         satisfies the specification given through 1-3.
+      5. Function expandBranch_sem_conform checks for all components declared anywhere
+         in a module whether expandBranch_fun satisfies the specification.
+         This function relies on CE.env to find which components are declared and their
+         types. (In particular, for instances this could not be done without a CE.env.) *)
+
+   Inductive expr_tree : Type :=
+   (* This data type describes the resulting value of a component depending on the execution path.
       Whenever there is a when statement (and the component has been declared before,
       so it is available in both execution paths), a T_choice node is inserted. *)
-   Inductive expr_tree : Type :=
    | T_undeclared (* in this execution path, the component is not declared *)
    | T_undefined (* the component is erroneously not connected *)
-   | T_invalidated (* the component is not connected but the programmer has indicated with an "is invalid" statement that this is ok *)
+   | T_invalidated (* the component is not connected but the programmer has
+                      indicated with an "is invalid" statement that this is ok *)
    | T_fexpr : hfexpr -> expr_tree
    | T_choice : hfexpr (* condition *) ->
                 expr_tree (* choice if condition is true *) ->
@@ -2075,109 +622,236 @@ Proof.
    match ss with
    | Qnil => default
    | Qcons s tl => match s with
-                   | @Sreg _ id _ => expandBranch_one_var_sem tl ref (if base_ref ref == id then T_fexpr (Eref ref) else default)
-                   | @Swire _ id _
-                   (* In the two lines below we disregard that some subfields of an instance may be flipped
+                   | @Sreg _ id _ => (* In the then branch, ref must refer to a ground element that is stored in the register *)
+                                     expandBranch_one_var_sem tl ref (if base_ref ref == id then T_fexpr (Eref ref) else default)
+                   (* In the three lines below we disregard that some subfields of a wire/instance may be flipped
                       and therefore have source flow direction; similarly, <memory id>.<read port id>.data
                       has source flow direction.  That is why we have the precondition
                       that ref must have sink (or duplex) flow direction. *)
                    | @Smem _ id _
+                   | @Swire _ id _
                    | @Sinst _ id _ => expandBranch_one_var_sem tl ref (if base_ref ref == id then T_undefined else default)
-                   (* In the two lines below we assume that ref0 is a ground type, as ExpandConnects has already been applied. *)
+                   (* In the two lines below we assume that ref0 is a ground type and not a subaccess, as ExpandConnects has already been applied. *)
                    | @Sfcnct _ ref0 expr => expandBranch_one_var_sem tl ref (if ref == ref0 then T_fexpr expr else default)
                    | @Sinvalid _ ref0 => expandBranch_one_var_sem tl ref (if ref == ref0 then T_invalidated else default)
-                   | @Swhen _ cond ss_true ss_false => let true_result  := expandBranch_one_var_sem ss_true  ref default in
-                                                       let false_result := expandBranch_one_var_sem ss_false ref default in
-                                                       match true_result, false_result with
-                                                       (* ignore execution paths where ref is not declared *)
-                                                       | T_undeclared, _ => expandBranch_one_var_sem tl ref false_result
-                                                       | _, T_undeclared => expandBranch_one_var_sem tl ref true_result
-                                                       | _, _ => expandBranch_one_var_sem tl ref
-                                                                 (if true_result == false_result then true_result
-                                                                  else T_choice cond true_result false_result)
-                                                       end
+                   | @Swhen _ cond ss_true ss_false => let true_result  := expandBranch_one_var_sem ss_true  ref default
+                                                       in let false_result := expandBranch_one_var_sem ss_false ref default
+                                                          in let result := match true_result, false_result with
+                                                                           (* ignore execution paths where ref is not declared *)
+                                                                           | T_undeclared, _ => expandBranch_one_var_sem tl ref false_result
+                                                                           | _, T_undeclared => expandBranch_one_var_sem tl ref true_result
+                                                                           | _, _ => expandBranch_one_var_sem tl ref
+                                                                                     (if true_result == false_result then true_result
+                                                                                      else T_choice cond true_result false_result)
+                                                                           end
+                                                             in expandBranch_one_var_sem tl ref result
                    | _ => expandBranch_one_var_sem tl ref default
                    end
    end.
 
    Fixpoint expr_tree_to_def_expr (tree: expr_tree) : option def_expr :=
-   (* This function translates a def-expression (that represents the value of a connect, depending on the execution path)
-      to a rhs_expr (which should be the output of the ExpandWhen phase for this reference) *)
+   (* This function translates an expression tree (that represents the value of a connect,
+      depending on the execution path) to a def_expr (which should be the output of the
+      ExpandWhen phase for this reference). *)
    match tree with
    | T_undeclared => None
    | T_undefined => Some D_undefined
    | T_invalidated => Some D_invalidated
    | T_fexpr e => Some (D_fexpr e)
-   | T_choice cond true_tree false_tree => let true_expr  := expr_tree_to_def_expr true_tree  in
-                                           let false_expr := expr_tree_to_def_expr false_tree in
-                                           match true_expr, false_expr with
-                                           | None, _
-                                           | _, Some D_undefined => false_expr
-                                           | _, None
-                                           | Some D_undefined, _
-                                           | Some D_invalidated, Some D_invalidated => true_expr
-                                           | Some (D_fexpr te), Some D_invalidated => Some (D_fexpr (Evalidif cond te))
-                                           | Some D_invalidated, Some (D_fexpr fe) => Some (D_fexpr (Evalidif (Eprim_unop Unot cond) fe))
-                                           | Some (D_fexpr te), Some (D_fexpr fe) => if te == fe then Some (D_fexpr te)
-                                                                                     else Some (D_fexpr (Emux cond te fe))
-                                           end
+   | T_choice cond true_tree false_tree => let true_expr := expr_tree_to_def_expr true_tree
+                                           in let false_expr := expr_tree_to_def_expr false_tree
+                                              in match true_expr, false_expr with
+                                                 | None, _
+                                                 | _, Some D_undefined => false_expr
+                                                 | _, None
+                                                 | Some D_undefined, _
+                                                 | Some D_invalidated, Some D_invalidated => true_expr
+                                                 | Some (D_fexpr te), Some D_invalidated => Some (D_fexpr (Evalidif cond te))
+                                                 | Some D_invalidated, Some (D_fexpr fe) => Some (D_fexpr (Evalidif (Eprim_unop Unot cond) fe))
+                                                 | Some (D_fexpr te), Some (D_fexpr fe) => if te == fe then Some (D_fexpr te)
+                                                                                           else Some (D_fexpr (Emux cond te fe))
+                                                 end
    end.
 
-   Definition expandBranch_vars_sem (ss : hfstmt_seq) (ce : cenv) (cm : cmap) (default : cmap) : Prop :=
-   (* Specification: If ce contains the types of components declared in ss, then cm contains the connects defined by ss.
-      If there is no connect, then the value of cm is copied from default. *)
+   Fixpoint expandBranch_one_component_sem_conform (ref : href) (t : ftype) (ss : hfstmt_seq) (cm : cmap) (default : cmap) : bool :=
+   (* This function checks for every ground element of component ref, which has type t,
+      whether cm satisfies the specification given by expandBranch_one_var_sem.
+      cm should contain the connects for the ground elements produced by
+      (ExpandBranch_fun ss ... default).
 
-   forall id : V.T, match CE.find id ce with
-                    | None => false
-                    | Some (t, _) => is_passive (type_of_cmpnttyp t)
-                    end ->
-                    let default_value := match CE.find id default with
-                                         | None => T_undeclared
-                                         | Some D_undefined => T_undefined
-                                         | Some D_invalidated => T_invalidated
-                                         | Some (D_fexpr e) => T_fexpr e
-                                         end in
-                    CE.find id cm == expr_tree_to_def_expr (expandBranch_one_var_sem ss (eid id) default_value).
-   (* Instead of Eid id in the line above, one should construct the (possibly structured) reference *)
+      It is assumed that ref has sink or duplex flow; flipped parts of ref are skipped.
+      ref is a wire (duplex flow), a memory port (sink flow), or an output port (sink flow).
+      Input ports (source flow) should be handled by the corresponding function for flipped data types.
+      For wires, one should call both this function and the one for flipped data types to get a complete verification. *)
+   match t with
+   | Gtyp _ => let default_value := match CE.find (ref2var ref) default with
+                                    | None => T_undeclared
+                                    | Some D_undefined => T_undefined
+                                    | Some D_invalidated => T_invalidated
+                                    | Some (D_fexpr e) => T_fexpr e
+                                    end
+               in CE.find (ref2var ref) cm == expr_tree_to_def_expr (expandBranch_one_var_sem ss ref default_value)
+   | Atyp t' array_size => [forall n: ordinal array_size, expandBranch_one_component_sem_conform (Esubindex ref n) t' ss cm default]
+   | Btyp ff => expandBranch_one_component_sem_conform_fields ref ff ss cm default
+   end
+   with expandBranch_one_component_sem_conform_fields (ref : href) (ff : ffield) (ss : hfstmt_seq) (cm : cmap) (default : cmap) : bool :=
+   match ff with
+   | Fnil => true
+   | Fflips f Nflip t' ff_tail =>    expandBranch_one_component_sem_conform (Esubfield ref f) t' ss cm default
+                                  && expandBranch_one_component_sem_conform_fields ref ff_tail ss cm default
+   | Fflips f Flipped t' ff_tail =>    expandBranch_one_component_sem_conform_flipped (Esubfield ref f) t' ss cm default
+                                    && expandBranch_one_component_sem_conform_fields ref ff_tail ss cm default
+   end
+   with expandBranch_one_component_sem_conform_flipped (ref : href) (t : ftype) (ss : hfstmt_seq) (cm : cmap) (default : cmap) : bool :=
+   (* This function checks for every ground element of component ref, which has type t,
+      whether cm satisfies the specification given by expandBranch_one_var_sem.
+      cm should contain the connects for the ground elements produced by
+      (ExpandBranch_fun ss ... default).
 
-   Fixpoint expandWhen_precondition_ss (ss : hfstmt_seq) : Prop :=
-   (* Precondition of expandWhen: there are no aggregate types and no partial connects *)
+      It is assumed that ref has source or duplex flow; only flipped parts of ref are checked.
+      ref is a wire (duplex flow) or an input port.
+      Memory ports and output port (sink flow) should be handled by the corresponding function for non-flipped data types.
+      For wires, one should call both this function and the one for non-flipped data types to get a complete verification. *)
+   match t with
+   | Gtyp _ => true (* no requirement on flipped parts / source flow parts *)
+   | Atyp t' array_size => [forall n: ordinal array_size, expandBranch_one_component_sem_conform_flipped (Esubindex ref n) t' ss cm default]
+   | Btyp ff => expandBranch_one_component_sem_conform_flipped_fields ref ff ss cm default
+   end
+   with expandBranch_one_component_sem_conform_flipped_fields (ref : href) (ff : ffield) (ss : hfstmt_seq) (cm : cmap) (default : cmap) : bool :=
+   match ff with
+   | Fnil => true
+   | Fflips f Nflip t' ff_tail =>    expandBranch_one_component_sem_conform_flipped (Esubfield ref f) t' ss cm default
+                                  && expandBranch_one_component_sem_conform_flipped_fields ref ff_tail ss cm default
+   | Fflips f Flipped t' ff_tail =>    expandBranch_one_component_sem_conform (Esubfield ref f) t' ss cm default
+                                    && expandBranch_one_component_sem_conform_flipped_fields ref ff_tail ss cm default
+   end.
+
+   Definition memory_readport_type (t : ftype) (addr_size : nat) : ftype :=
+   Btyp (Fflips mem_port_addr Nflip (Gtyp (Fuint addr_size))
+        (Fflips mem_port_en Nflip (Gtyp (Fuint 1))
+        (Fflips mem_port_clk Nflip (Gtyp Fclock)
+        (Fflips mem_port_data Flipped t Fnil)))).
+
+   Fixpoint mask_type (t : ftype) : ftype :=
+   (* the type of the mask field of a write port of a memory with type t *)
+   match t with
+   | Gtyp _ => Gtyp (Fuint 1)
+   | Atyp t n => Atyp (mask_type t) n
+   | Btyp ff => Btyp (mask_type_fields ff)
+   end
+   with mask_type_fields (ff : ffield) : ffield :=
+   match ff with
+   | Fnil => Fnil
+   | Fflips fieldname Nflip t ff_tail => Fflips fieldname Nflip (mask_type t) (mask_type_fields ff_tail)
+   | Fflips fieldname Flipped t ff_tail => Fnil (* error *)
+   end.
+
+   Definition memory_writeport_type (t : ftype) (addr_size : nat) : ftype :=
+   Btyp (Fflips mem_port_addr Nflip (Gtyp (Fuint addr_size))
+        (Fflips mem_port_en Nflip (Gtyp (Fuint 1))
+        (Fflips mem_port_clk Nflip (Gtyp Fclock)
+        (Fflips mem_port_data Nflip t
+        (Fflips mem_port_mask Nflip (mask_type t) Fnil))))).
+
+   Fixpoint expandBranch_readports_sem_conform (m_id : VarOrder.t) (addr_size : nat) (readports : seq mem_port) (t : ftype)
+                                               (ss : hfstmt_seq) (cm : cmap) (default : cmap) : bool :=
+   match readports with
+   | [::] => true
+   | rp :: readports_tail =>    expandBranch_one_component_sem_conform (Esubfield (Eid m_id) (id rp))
+                                                  (memory_readport_type t addr_size) ss cm default
+                             && expandBranch_readports_sem_conform m_id addr_size readports_tail t ss cm default
+   end.
+
+   Fixpoint expandBranch_writeports_sem_conform (m_id : VarOrder.t) (addr_size : nat) (writeports : seq mem_port) (t : ftype)
+                                               (ss : hfstmt_seq) (cm : cmap) (default : cmap) : bool :=
+   match writeports with
+   | [::] => true
+   | wp :: writeports_tail =>    expandBranch_one_component_sem_conform (Esubfield (Eid m_id) (id wp))
+                                                   (memory_writeport_type t addr_size) ss cm default
+                              && expandBranch_writeports_sem_conform m_id addr_size writeports_tail t ss cm default
+   end.
+
+   Definition expandBranch_memory_sem_conform (id : var) (m : hfmem) (ss : hfstmt_seq) (cm : cmap) (default : cmap) : bool :=
+   (* This adapter function calls the appropriate variants of expandBranch_one_component_sem_conform
+      for memory defined by id. It basically goes through all ports and checks their interfaces. *)
+   let addr_size := if depth m <=? 1 then 0 else Nat.log2 (depth m - 1) + 1
+   in    expandBranch_readports_sem_conform  id addr_size (reader m) (data_type m) ss cm default
+      && expandBranch_writeports_sem_conform id addr_size (writer m) (data_type m) ss cm default
+   .
+
+   Definition expandBranch_sem_conform_helper (ss : hfstmt_seq) (cm : cmap) (default : cmap)
+                                     (id : VarOrder.T) (def : cmpnt_init_typs * fcomponent) (val: bool) : bool :=
+   (* This helper function verifies for all ground elements of component id, which is of type and kind def,
+      whether cm satisfies the specification given by expandBranch_one_var_sem.
+      cm should contain the connects for the ground elements produced by
+      (ExpandBranch_fun ss ... default). *)
+   val && match def with
+          | (Aggr_typ t, Wire) =>    expandBranch_one_component_sem_conform (Eid id) t ss cm default
+                                  && expandBranch_one_component_sem_conform_flipped (Eid id) t ss cm default
+          | (Aggr_typ t, Instanceof)
+          | (Aggr_typ t, In_port) => expandBranch_one_component_sem_conform_flipped (Eid id) t ss cm default
+          | (Aggr_typ t, Out_port) => expandBranch_one_component_sem_conform (Eid id) t ss cm default
+          | (Reg_typ r, Register) => expandBranch_one_component_sem_conform (Eid id) (type r) ss cm default
+          | (Mem_typ m, Memory) => expandBranch_memory_sem_conform id m ss cm default
+          | _ => false (* error *)
+          end.
+
+   Fixpoint expandWhen_precondition_ss (ss : hfstmt_seq) (ce : CE.env) : bool :=
+   (* Precondition of expandWhen: there are no partial connects *)
    match ss with
-   | Qnil => True
+   | Qnil => true
    | Qcons s tl => match s with
-                  | @Spcnct _ _ _ => False
-                  | @Sfcnct _ v _ => match v with Eid _ => expandWhen_precondition_ss tl
-                                                | _ => False end
-                  | @Swhen _ _ sst ssf =>    expandWhen_precondition_ss sst
-                                          /\ expandWhen_precondition_ss ssf
-                                          /\ expandWhen_precondition_ss tl
-                  | _ => expandWhen_precondition_ss tl
+                  | Spcnct _ _ => false
+                  | Sinst id def => if CE.find def ce is Some (_, Fmodule) then expandWhen_precondition_ss tl ce else false
+                  | Swhen _ sst ssf =>    expandWhen_precondition_ss sst ce
+                                          && expandWhen_precondition_ss ssf ce
+                                          && expandWhen_precondition_ss tl ce
+                  | _ => expandWhen_precondition_ss tl ce
                   end
    end.
 
-   Fixpoint expandWhen_ce (ss : hfstmt_seq) (default : cenv) : cenv :=
-   (* ce contains exactly the component types as defined by ss, in addition to default. *)
+   Fixpoint expandWhen_ce (ss : hfstmt_seq) (ce : CE.env) (default : CE.env) : CE.env :=
+   (* The result contains exactly the component types as defined by ss, in addition to default.
+      The parameter ce contains the port declarations of other modules. *)
    match ss with
    | Qnil => default
    | Qcons s ss_tail => match s with
-                        | Sskip => expandWhen_ce ss_tail default
-                        | Swire id t => expandWhen_ce ss_tail (CE.add id (@Aggr_typ V.T t, Wire) default)
-                        | Sreg id reg => expandWhen_ce ss_tail (CE.add id (Reg_typ reg, Register) default)
-                        | Smem id mem => expandWhen_ce ss_tail (CE.add id (Mem_typ mem, Memory) default)
-                        | Sinst typ id => CE.empty (cmpnt_init_typs * fcomponent) (* TBD *)
+                        | Swire id t => expandWhen_ce ss_tail ce (CE.add id (@Aggr_typ VarOrder.T t, Wire) default)
+                        | Sreg id reg => expandWhen_ce ss_tail ce (CE.add id (Reg_typ reg, Register) default)
+                        | Smem id mem => expandWhen_ce ss_tail ce (CE.add id (Mem_typ mem, Memory) default)
+                        | Sinst id typ => expandWhen_ce ss_tail ce (CE.add id (fst (CE.vtyp typ ce), Instanceof) default)
+                        | Sskip
                         | Snode _ _ (* can be ignored *)
                         | Sfcnct _ _
-                        | Spcnct _ _ (* should not appear *)
-                        | Sinvalid _ => expandWhen_ce ss_tail default
-                        | Swhen _ ss_true ss_false => expandWhen_ce ss_tail (expandWhen_ce ss_false (expandWhen_ce ss_true default))
-                        | Sstop _ _ _ => expandWhen_ce ss_tail default
+                        | Sinvalid _ => expandWhen_ce ss_tail ce default
+                        | Swhen _ ss_true ss_false => expandWhen_ce ss_tail ce (expandWhen_ce ss_false ce (expandWhen_ce ss_true ce default))
+                        (* | Sstop _ _ _ => expandWhen_ce ss_tail default *)
+                        | Spcnct _ _ (* error: should not appear *) => CE.empty (cmpnt_init_typs * fcomponent)
                         end
    end.
+
+   Definition expandBranch_sem_conform (mdl : hfmodule) (ce : CE.env) : bool :=
+   (* Checks for all components declared in module mdl
+      whether expandBranch_fun satisfies the specification.
+      * mdl = module to be checked
+      * ce = component environment containing all port declarations of other modules *)
+   match mdl with
+   | FInmod _ ports ss => expandWhen_precondition_ss ss ce ==>
+                          let ports_cmap := init_ports ports empty_cmap
+                          in CE.fold (expandBranch_sem_conform_helper ss (snd (expandBranch_fun ss ce ports_cmap)) ports_cmap)
+                                     (expandWhen_ce ss ce (CE.empty (cmpnt_init_typs * fcomponent))) true
+   | FExmod _ _ _ => false (* error *)
+   end.
+
+(* How to prove the correctness of this semantics?
+   Basically, we would like to show that for every correct (hfmodule * CE.env) pair,
+   we have that expandBranch_sem_conform returns true.
+   Preconditions are, in addition to expandWhen
 
    Definition expandBranch_hfstmt_seq_sem_conform (ss : hfstmt_seq) : Prop :=
    (* The statements in ss are being translated by expandBranch_fun to correct definitions in a cmap. *)
       expandWhen_precondition_ss ss ->
-      forall ce : cenv, ce = expandWhen_ce ss (CE.empty (cmpnt_init_typs * fcomponent)) ->
+      forall ce : CE.env, ce = expandWhen_ce ss (CE.empty (cmpnt_init_typs * fcomponent)) ->
                         forall default : cmap, expandBranch_vars_sem ss ce (snd (expandBranch_fun ss ce default None)) default.
 
    Definition expandBranch_hfstmt_sem_conform (s : hfstmt) : Prop :=
@@ -2599,8 +1273,8 @@ Proof.
     | _, _ => None
     end.
 
-   (* Fixpoint try_expandBranch_fun (s :  hfstmt) (ce : cenv) (cs : cstate) {struct s}: (cstate):= *)
-   (*        let fix aux (ss : seq hfstmt) (ce : cenv) (cs : cstate) {struct ss}: (cstate) := *)
+   (* Fixpoint try_expandBranch_fun (s :  hfstmt) (ce : CE.env) (cs : cstate) {struct s}: (cstate):= *)
+   (*        let fix aux (ss : seq hfstmt) (ce : CE.env) (cs : cstate) {struct ss}: (cstate) := *)
 
    (*            match ss with *)
    (*            | [::] => (cs) *)
@@ -2618,7 +1292,7 @@ Proof.
    (*                                                                   The above code works for registers of basic type. *) *)
    (*               | Smem v m =>  cs (* but should assign R_default to all *)
    (*                                                                      input signals of ports *) *)
-   (*               | Swire v t => SV.upd v (R_default V.T) cs *)
+   (*               | Swire v t => SV.upd v (R_default VarOrder.T) cs *)
    (*               | Sfcnct v e => SV.upd (expand_eref v ce) (R_fexpr e) cs *)
    (*               | Swhen c sst ssf => let combined_branches := SV.map2 (merge_branch_cs_t c) (aux sst ce cs) (aux ssf ce cs) in *)
    (*                                    (* let result := try_expandBranch_fun s ce (snd combined_branches) in *) *)
@@ -2715,288 +1389,3 @@ Proof.
   (* Lemma valid_conncection v e2 sts ce cs ce' cs' : *)
   (*   eval_fstmts_group (Qcons (sfcnct (eref v) e2) sts) ce cs ce' cs' -> *)
   (*   valid_rhs (SV.acc v cs') ce'. *)
-
-(* COMMENT OUT END HERE *)
-*)
-
-End MakeHiFirrtl.
-
-(********************************************************************************)
-
-
-(* HiFirrtl module with variables of type N *)
-Module HiF := MakeHiFirrtl VarOrder (* ProdVarOrder PVS *) VS VM CE StructState (* CEP StructStateP *).
-
-
-
-
-Module MakeHiFirrtlP
-  (V : SsrOrder) (* identifier names *)
-  (PVS : SsrFSet with Module SE := V)
-  (PVM : SsrFMap with Module SE := V)
-  (PCE : CmpntEnv V with Module SE := V)
-  (PSV : StructStore V PCE). 
-
-
-  Module PCELemmas := FMapLemmas PCE.
-  Module PVSLemmas := SsrFSetLemmas PVS.
-
-  Local Notation pvar := (V.t * V.t).
-
-  Local Notation pcstate := PSV.t.
-  Local Notation pcenv := PCE.env. 
-
-  Definition econst s c := @Econst V.T s c.
-  Definition ecast u e := @Ecast V.T u e.
-  Definition eprim_unop u e := @Eprim_unop V.T u e.
-  Definition eprim_binop b e1 e2 := @Eprim_binop V.T b e1 e2.
-  Definition emux c e1 e2 := @Emux V.T c e1 e2.
-  Definition evalidif c e := @Evalidif V.T c e.
-  Definition hfexpr := hfexpr V.T.
-  Definition eref r := @Eref V.T r.
-  Definition eid v := @Eid V.T v.
-  Definition esubfield r v := @Esubfield V.T r v.
-  Definition esubindex r n := @Esubindex V.T r n.
-  Definition esubaccess r e := @Esubaccess V.T r e.
-  Definition href := href V.T.
-
-  Definition hfstmt := hfstmt V.T.
-  Definition hfstmt_seq := hfstmt_seq V.T.
-  Definition qnil := Qnil V.T.
-(*Definition qcons s ss := @Qcons V.T s ss.*)
-  Definition sskip := @Sskip V.T.
-  Definition swire v t := @Swire V.T v t.
-  Definition sreg v r := @Sreg V.T v r.
-  Definition smem v m := @Smem V.T v m.
-  Definition snode v e := @Snode V.T v e.
-  Definition sfcnct v1 v2 := @Sfcnct V.T v1 v2.
-  Definition spcnct v1 v2 := @Spcnct V.T v1 v2.
-  Definition sinvalid v1 := @Sinvalid V.T v1.
-  Definition swhen c s1 s2 := @Swhen V.T c s1 s2.
-  (* Definition sstop e1 e2 n := @Sstop V.T e1 e2 n. *)
-  Definition sinst v1 v2 := @Sinst V.T v1 v2.
-
-  Definition hfreg := @hfreg V.T.
-  Definition mk_hfreg := @mk_freg V.T.
-  Definition nrst := @NRst V.T.
-  Definition rrst e1 e2 := @Rst V.T e1 e2.
-  Definition mk_mem_port := @mk_mem_port V.T.
-  Definition mem_port := @mem_port V.T.
-  Definition hfmem := @hfmem V.T.
-  Definition mk_hfmem := @mk_fmem V.T.
-  Definition hfport := @hfport V.T.
-  Definition hinport v t := @Finput V.T v t.
-  Definition houtport v t := @Foutput V.T v t.
-  Definition hfmodule := @hfmodule V.T.
-  Definition hfinmod v ps ss := @FInmod V.T v ps ss.
-  Definition hfexmod v ps ss := @FExmod V.T v ps ss.
-  Definition hfcircuit := @hfcircuit V.T.
-
-  Definition rhs_expr := rhs_expr V.T.
-  Definition r_fexpr e := @R_fexpr V.T e.
-  Definition r_default := @R_default V.T.
-
-  Definition cmpnt_init_typs := @cmpnt_init_typs V.T.
-  Definition aggr_typ t := @Aggr_typ V.T t.
-  Definition reg_typ t := @Reg_typ V.T t.
-  Definition mem_typ t := @Mem_typ V.T t.
-  Definition unknown_typ := @Unknown_typ V.T.
-  
-End MakeHiFirrtlP.
-
-Module HiFP := MakeHiFirrtlP ProdVarOrder PVS PVM CEP StructStateP.
-
-
-(* idents pair *)
-Definition pvar := ProdVarOrder.t.
-Definition def_pvar := ProdVarOrder.default.
-
-Section Preprocess.
-  
-  (* index *)
-  Definition initial_index : N := 0.
-  Definition first_index : N := 1.
-  
-  (* generator stores the next starting point *)
-  Definition generator := N.
-  (* ig contain fst as next ident index, snd as current index *)
-  Definition index_gen (g : generator * N) ft : (generator * N) := (N.add (fst g) (N.of_nat (size_of_ftype ft)), (fst g)).
-  Definition newer_than_current (g: generator * N) : bool := N.ltb (snd g) (fst g).
-  Definition new_index_gen (g : generator) ft : generator :=
-    let s := (size_of_ftype ft) in
-    if s==0 then N.add g 1
-    else
-      N.add g (N.of_nat (size_of_ftype ft).+1).
-
-  (* A map from paired vars to eref *) Print href.
-  Definition eids := (href ProdVarOrder.T).
-   Definition eid v := @Eid ProdVarOrder.T v. 
-  Definition esubfield r v := @Esubfield ProdVarOrder.T r v.
-  Definition esubindex r n := @Esubindex ProdVarOrder.T r n.
-  Definition esubaccess r e := @Esubaccess ProdVarOrder.T r e.
-  Definition hfstmt' := (@hfstmt ProdVarOrder.T).
-  Definition hfstmt_seq' := hfstmt_seq ProdVarOrder.T.
-  Definition qnil := Qnil ProdVarOrder.T.
-(*Definition qcons s ss' := @Qcons VarOrder.T s ss.*)
-  Definition sskip := @Sskip ProdVarOrder.T.
-  Definition swire v t := @Swire ProdVarOrder.T v t.
-  Definition sreg v r := @Sreg ProdVarOrder.T v r.
-  Definition smem v m := @Smem ProdVarOrder.T v m.
-  Definition snode v e := @Snode ProdVarOrder.T v e.
-  Definition sfcnct v1 v2 := @Sfcnct ProdVarOrder.T v1 v2.
-  Definition spcnct v1 v2 := @Spcnct ProdVarOrder.T v1 v2.
-  Definition sinvalid v1 := @Sinvalid ProdVarOrder.T v1.
-  Definition swhen c s1 s2 := @Swhen ProdVarOrder.T c s1 s2.
-  (* Definition sstop e1 e2 n := @Sstop VarOrder.T e1 e2 n. *)
-  Definition sinst v1 v2 := @Sinst ProdVarOrder.T v1 v2.
-  
-  Definition eid_map := PVM.t HiF.href.
-  Definition eid_map_empty : eid_map := PVM.empty HiF.href.
-
-  (* finds/acc in eid_map*)  
-  Definition acc_indexes (m:eid_map) (v:pvar): HiF.href :=
-    match PVM.find v m with
-    | Some i => i
-    | None => HiF.eid (initial_index)
-    end.
-
-  (* generator generates newer index*)
-  Definition gen_newer_than (g: generator * N) (m : eid_map) :=
-    forall v rs, PVM.find v m = Some rs -> N.ltb (fst v) (fst g).
-
-  Definition offset_ref r ce: N:=
-    match r with
-    | Eid v => 0
-    | Esubfield r1 v => N.of_nat (offset_of_subfield (HiF.type_of_hfexpr (HiF.eref r) ce) v 0)
-    | Esubindex r1 n => N.of_nat (offset_of_subindex (HiF.type_of_hfexpr (HiF.eref r) ce) n)
-    | _ => 0
-    end.
-
-  Fixpoint expr_pvar (em : eid_map) (ce : CE.env) (h : HiF.hfexpr) : HiFP.hfexpr :=
-    match h with
-    | Econst t b => HiFP.econst t b
-    | Ecast u e => HiFP.ecast u (expr_pvar em ce e)
-    | Eprim_unop u e => HiFP.eprim_unop u (expr_pvar em ce e)
-    | Eprim_binop b e1 e2 => HiFP.eprim_binop b (expr_pvar em ce e1) (expr_pvar em ce e2)
-    | Emux e1 e2 e3 => HiFP.emux (expr_pvar em ce e1) (expr_pvar em ce e2) (expr_pvar em ce e3)
-    | Evalidif e1 e2 => HiFP.evalidif (expr_pvar em ce e1) (expr_pvar em ce e2)
-    | Eref r => HiFP.eref (HiFP.eid (HiF.base_ref r, offset_ref r ce))
-    end.
-
-  (* Parameter rst_pvar : HiF.rst -> HiFP.rst. *)
-  
-  Parameter hfreg_pvar: HiF.hfreg -> HiFP.hfreg.
-    (* HiFP.mk_hfreg (type r) (clock (expr_pvar (clock h))) () *)
-  Parameter hfmem_pvar: HiF.hfmem -> HiFP.hfmem.
-  
-  Fixpoint hfstmt_indexes (* (g : generator) *) (em : eid_map) (ce : CE.env) (h : HiF.hfstmt) : (* generator **) eid_map * CE.env * hfstmt' :=
-    match h with
-    | Swire v t => ((* new_index_gen g t, *) PVM.add (v, initial_index) (HiF.eid v) em, CE.add v (HiF.aggr_typ t, Wire) ce, swire (v, initial_index) t)
-    | Sreg v r => ((* new_index_gen g (type r), *) PVM.add (v, initial_index) (HiF.eid v) em, CE.add v (HiF.reg_typ r, Register) ce, sreg (v, initial_index) (hfreg_pvar r))
-    | Smem v m => ( PVM.add (v, initial_index) (HiF.eid v) em, CE.add v (HiF.mem_typ m, Memory) ce, smem (v, initial_index) (hfmem_pvar m)) 
-    | Sinst v1 v2 => ( PVM.add (v1, initial_index) (HiF.eid v1) em, CE.add v1 ((fst (CE.vtyp v2 ce)), Instanceof) ce, sinst (v1, initial_index) (v2, initial_index))
-    | Snode v e => ( PVM.add (v, initial_index) (HiF.eid v) em, CE.add v (HiF.aggr_typ (HiF.type_of_hfexpr e ce), Node) ce, snode (v, initial_index) (expr_pvar em ce e))
-    | Sfcnct r e => (PVM.add (HiF.base_ref r, offset_ref r ce) (r) em, ce, sfcnct ( (HiFP.eid (HiF.base_ref r, (offset_ref r ce)))) (expr_pvar em ce e))
-    | Spcnct r e => (PVM.add (HiF.base_ref r, offset_ref r ce) (r) em, ce, spcnct ( (HiFP.eid (HiF.base_ref r, (offset_ref r ce)))) (expr_pvar em ce e))
-    | Sinvalid r => (PVM.add (HiF.base_ref r, offset_ref r ce) (r) em, ce, sinvalid ( (HiFP.eid (HiF.base_ref r, (offset_ref r ce)))))
-    | Swhen e s1 s2 => (em, ce, swhen (expr_pvar em ce e) (snd (hfstmt_seq_indexes em ce s1)) (snd (hfstmt_seq_indexes em ce s2)))
-    | Sskip => ( em, ce, sskip)
-    end
-  with hfstmt_seq_indexes em ce s : eid_map * CE.env * HiFP.hfstmt_seq :=
-         match s with
-         | Qnil => (em, ce, HiFP.qnil)
-         | Qcons s ss => hfstmt_seq_indexes (fst (fst (hfstmt_indexes em ce s))) (snd (fst (hfstmt_indexes em ce s))) ss
-    end.
-  
-  (* A map from paired vars to index *)
-  Definition ind_map := PVM.t (N * N).
-  Definition ind_map_empty : ind_map := PVM.empty (N * N).
-
-  (* finds/acc in idents_map*)
-  Definition find_base_index (m:ind_map) (v:pvar): option N :=
-    match PVM.find v m with
-    | Some i => Some (fst i)
-    | None => None
-    end.
-
-  Definition find_offset_index (m:ind_map) (v:pvar): option N :=
-    match PVM.find v m with
-    | Some i => Some (snd i)
-    | None => None
-    end.
-  
-  (* set/get index with base and offset index*)
-  Definition upd_ind_map (v:pvar) (m:ind_map) (ig : generator * N) ft: ind_map * (generator * N):=
-    match PVM.find v m with
-    | Some i => (m, ig)
-    | None => let idg := index_gen ig ft in (PVM.add v (snd ig, initial_index) m, idg)
-    end.
-
-  Definition newer_than (g: generator * N) (m : ind_map) :=
-  forall v rs, PVM.find v m = Some rs -> N.ltb (fst g) (fst rs).
-  
-  (* Parameter get_set_pvar : forall m (p:pvar), acc_indexes m p = p. *)
-  
-  (* Definition get_pvar m (p:pvar) : N * N := ((acc_indexes m p).1%N, (acc_indexes m p).2%N). *)
-
-  
-  
-  (* Lemma pvar_preserve1 (m : ind_map) : Ids_map2.preserve (get_pvar m). *)
-  (* Proof. *)
-  (*   move => x y H. *)
-  (*   rewrite (eqP H) eq_refl//. *)
-  (* Qed. *)
-
-  (* Lemma pvar_injective1 (m : ind_map) : Ids_map2.injective (get_pvar m). *)
-  (* Proof. *)
-  (*   move => x y /eqP H.  *)
-  (*   case : H. *)
-  (*   rewrite !get_set_pvar. *)
-  (*   case x => x1 x2; case y => y1 y2 => /= H1 H2. *)
-  (*   rewrite H1 H2//. *)
-  (* Qed. *)
-
-  (* Definition pvar_well m := *)
-  (*   Ids_map2.mkWellMap2 (pvar_preserve1 m) (pvar_injective1 (m:=m)). *)
-
-  (* (* Change var to idents in statements *) *)
-  (* Definition make_fstmt_ids st := *)
-  (*   match st with *)
-  (*   | Swire v t =>  *)
-  
-
-  (* (* A map from paired indexes to single index *) *)
-  (* Definition sind_map := PVM.t N . *)
-  (* Definition sind_map_empty : sind_map := PVM.empty N. *)
-
-  (* Definition get_sind (v : pvar) (m : sind_map) : N := *)
-  (*   match PVM.find v m with *)
-  (*   | None => initial_index *)
-  (*   | Some i => i *)
-  (*   end. *)
-
-  (* (* Definition set_sind (v : pvar) (m : sind_map) : sind_map := *) *)
-  (* (*   match PVM.find v m with *) *)
-  (* (*   | Some i =>  *) *)
-  
-  (* Definition get_svar m (p:pvar) : N := N.add (acc_indexes m p).1%N (acc_indexes m p).2%N. *)
-
-  (* (* Lemma pvar_svar_preserve (m : sind_map) : Ids_id_map2.preserve (get_svar m). *) *)
-  (* (* Proof. *) *)
-  (* (*   move => x y H. *) *)
-  (* (*   rewrite (eqP H) eq_refl//. *) *)
-  (* (* Qed. *) *)
-
-  (* (* Lemma pvar_svar_injective (m : ind_map) : Ids_id_map2.injective (get_svar m). *) *)
-  (* (* Proof. *) *)
-  (* (*   move => x y /eqP H.  *) *)
-  (* (*   case : H. *) *)
-  (* (* Admitted. *) *)
-
-  (* (* Definition svar_well m := *) *)
-  (* (*   Ids_id_map2.mkWellMap2 (pvar_svar_preserve m) (pvar_svar_injective (m:=m)). *) *)
-  
-End Preprocess.
-
-  
-
